jwnlgj

.lake/build/ir/Games/gameLib/Pairing.c
@@ -1,6 +1,6 @@
 // Lean compiler output
 // Module: Games.gameLib.Pairing
-// Imports: Init Games.gameLib.Basic
+// Imports: Init Games.gameLib.Positional
 #include <lean/lean.h>
 #if defined(__clang__)
 #pragma clang diagnostic ignored "-Wunused-parameter"
@@ -13,8 +13,53 @@
 #ifdef __cplusplus
 extern "C" {
 #endif
+LEAN_EXPORT lean_object* l___private_Games_gameLib_Pairing_0__Game__World_hist__on__turn_match__1_splitter(lean_object*);
+LEAN_EXPORT lean_object* l___private_Games_gameLib_Pairing_0__Game__World_hist__on__turn_match__1_splitter___rarg(lean_object*, lean_object*, lean_object*);
+LEAN_EXPORT lean_object* l___private_Games_gameLib_Pairing_0__Game__World_hist__on__turn_match__1_splitter___rarg___boxed(lean_object*, lean_object*, lean_object*);
+uint8_t lean_nat_dec_eq(lean_object*, lean_object*);
+lean_object* lean_nat_sub(lean_object*, lean_object*);
+LEAN_EXPORT lean_object* l___private_Games_gameLib_Pairing_0__Game__World_hist__on__turn_match__1_splitter___rarg(lean_object* x_1, lean_object* x_2, lean_object* x_3) {
+_start:
+{
+lean_object* x_4; uint8_t x_5; 
+x_4 = lean_unsigned_to_nat(0u);
+x_5 = lean_nat_dec_eq(x_1, x_4);
+if (x_5 == 0)
+{
+lean_object* x_6; lean_object* x_7; lean_object* x_8; 
+x_6 = lean_unsigned_to_nat(1u);
+x_7 = lean_nat_sub(x_1, x_6);
+x_8 = lean_apply_1(x_3, x_7);
+return x_8;
+}
+else
+{
+lean_dec(x_3);
+lean_inc(x_2);
+return x_2;
+}
+}
+}
+LEAN_EXPORT lean_object* l___private_Games_gameLib_Pairing_0__Game__World_hist__on__turn_match__1_splitter(lean_object* x_1) {
+_start:
+{
+lean_object* x_2; 
+x_2 = lean_alloc_closure((void*)(l___private_Games_gameLib_Pairing_0__Game__World_hist__on__turn_match__1_splitter___rarg___boxed), 3, 0);
+return x_2;
+}
+}
+LEAN_EXPORT lean_object* l___private_Games_gameLib_Pairing_0__Game__World_hist__on__turn_match__1_splitter___rarg___boxed(lean_object* x_1, lean_object* x_2, lean_object* x_3) {
+_start:
+{
+lean_object* x_4; 
+x_4 = l___private_Games_gameLib_Pairing_0__Game__World_hist__on__turn_match__1_splitter___rarg(x_1, x_2, x_3);
+lean_dec(x_2);
+lean_dec(x_1);
+return x_4;
+}
+}
 lean_object* initialize_Init(uint8_t builtin, lean_object*);
-lean_object* initialize_Games_gameLib_Basic(uint8_t builtin, lean_object*);
+lean_object* initialize_Games_gameLib_Positional(uint8_t builtin, lean_object*);
 static bool _G_initialized = false;
 LEAN_EXPORT lean_object* initialize_Games_gameLib_Pairing(uint8_t builtin, lean_object* w) {
 lean_object * res;
@@ -23,7 +68,7 @@ _G_initialized = true;
 res = initialize_Init(builtin, lean_io_mk_world());
 if (lean_io_result_is_error(res)) return res;
 lean_dec_ref(res);
-res = initialize_Games_gameLib_Basic(builtin, lean_io_mk_world());
+res = initialize_Games_gameLib_Positional(builtin, lean_io_mk_world());
 if (lean_io_result_is_error(res)) return res;
 lean_dec_ref(res);
 return lean_io_result_mk_ok(lean_box(0));
