Games/gameLib/StateAPI.lean
@@ -5,7 +5,7 @@ Author: Yves Jäckle.
 -/
 
 import Games.gameLib.HistoryAPI
-
+import Games.gameLib.Termination
 
 lemma Game_World.state_on_turn_eq_state_from_hist (g : Game_World α β)
   {fst_strat : g.fStrategy} {snd_strat : g.sStrategy}
@@ -22,3 +22,53 @@ lemma Game_World.state_on_turn_eq_state_from_hist (g : Game_World α β)
     · dsimp [state_from_hist]
       simp_rw [hist_on_turn_length]
       rw [if_neg T]
+
+def State_from_history (ini : α ) (f_trans s_trans : List β → (β → α)) : List β → α
+| [] => ini
+| a :: h => if Turn_fst (h.length +1)
+            then f_trans h a
+            else s_trans h a
+
+lemma Game_World.state_on_turn_State_from_history (g : Game_World α β)
+    (fst_strat : g.fStrategy) (snd_strat : g.sStrategy)
+    (t : ℕ) :
+    g.state_on_turn fst_strat snd_strat t =
+    State_from_history g.init_game_state g.fst_transition g.snd_transition
+    (g.hist_on_turn fst_strat snd_strat t).val :=
+    by
+    cases' t with t
+    · dsimp!
+    · dsimp [state_on_turn, hist_on_turn]
+      split_ifs with T
+      · dsimp [State_from_history]
+        simp_rw [hist_on_turn_length]
+        rw [if_pos T]
+      · dsimp [State_from_history]
+        simp_rw [hist_on_turn_length]
+        rw [if_neg T]
+
+
+def State_from_history_neutral_wDraw (ini : α ) (f_wins s_wins draw : List β → Prop) (hist : List β) : Prop :=
+  (¬ (f_wins hist)) ∧ (¬ (s_wins hist) ∧ (¬ (draw hist)))
+
+
+lemma Game_World_wDraw.state_on_turn_neutral_State_from_history_neutral (g : Game_World_wDraw α β)
+  (f_strat : g.fStrategy) (s_strat : g.sStrategy) (turn : ℕ) :
+  g.state_on_turn_neutral f_strat s_strat turn ↔
+  State_from_history_neutral_wDraw g.init_game_state g.fst_win_states g.snd_win_states g.draw_states
+  (g.hist_on_turn f_strat s_strat turn).val :=
+  by
+  dsimp [Game_World_wDraw.state_on_turn_neutral, State_from_history_neutral_wDraw]
+  rw [← not_or, ← not_or, not_iff_not]
+  constructor
+  · intro h
+    cases' h with F S D
+    · left ; exact F
+    · right ; left ; exact S
+    · right ; right ; exact D
+  · intro h
+    cases' h with F O
+    · apply Game_World_wDraw.Turn_isWLD.wf ; exact F
+    · cases' O with S D
+      · apply Game_World_wDraw.Turn_isWLD.ws ; exact S
+      · apply Game_World_wDraw.Turn_isWLD.drw ; exact D
