Games/gameLib/Pairing.lean
@@ -1,0 +1,1384 @@
+/-
+Copyright (c) 2024 Yves Jäckle. All rights reserved.
+Released under Apache 2.0 license as described in the file LICENSE.
+Author: Yves Jäckle.
+-/
+
+import Games.gameLib.Positional
+
+
+/-
+This file is in dire need of cleaning.
+
+The file describes the notion of pairing stratgies for positional games.
+If there are pairs of tiles for each winning set, that are all distinct
+(wihtin and among pairs), then we can play as follows: if the opponent
+colors one of the pair elements on one turn, color the other on the next turn.
+This way, no winning set can become monochromatic, hence the game will end in a
+draw in the worst case for either player.
+
+The main concepts of the file are:
+- `Pairing_condition` is the condition for pairing strategies to exist
+- `Pairing_StratCore` is the core pairing strategy, which can be use by
+  either the first or the second player.
+- `Pairing_Strategy` is the theorem that states that if the pairing strat
+  conditionas are satisfied, the game ends in a draw in the worst case
+  (currently, only for the second player)
+
+-/
+
+
+
+structure pairProp {win_sets : Finset (Finset α)} (win_set : win_sets) (p : α × α) : Prop where
+  dif : p.1 ≠ p.2
+  mem_fst : p.1 ∈ win_set.val
+  mem_snd : p.2 ∈ win_set.val
+
+
+structure pairDif (a b : α × α) : Prop where
+  strait_fst : a.1 ≠ b.1
+  strait_snd : a.2 ≠ b.2
+  cross_fst : a.1 ≠ b.2
+  cross_snd : a.2 ≠ b.1
+
+structure Pairing_condition [DecidableEq α] [Fintype α] (win_sets : Finset (Finset α)) (pairing : win_sets → (α × α)) where
+  has_pairing : ∀ w : win_sets, pairProp w (pairing w)
+  pairing_dif : ∀ w v : win_sets, w ≠ v → pairDif (pairing w) (pairing v)
+
+
+
+noncomputable
+def Pairing_StratCore [Inhabited α] [DecidableEq α] [Fintype α] (win_sets : Finset (Finset α)) (pairing : win_sets → (α × α)) :
+  (hist : List α) → (leg : (Positional_Game_World win_sets).hist_legal hist) → α :=
+  fun hist leg =>
+    let spam :=
+      if T : Turn_fst (hist.length + 1)
+            then
+              Classical.choose (((Positional_Game_World_playable win_sets) hist (leg)).1 T)
+            else
+              Classical.choose (((Positional_Game_World_playable win_sets) hist (leg)).2 (by rw [Turn_snd_iff_not_fst] ; exact T))
+    match hist with
+    | last :: _ =>
+        if hxf : ∃ w : win_sets, last = (pairing w).1
+        then
+          let other := (pairing (Classical.choose hxf)).2
+          if other ∈ hist
+          then spam
+          else other
+        else
+          if hxs : ∃ w : win_sets, last = (pairing w).2
+          then
+            let other := (pairing (Classical.choose hxs)).1
+            if other ∈ hist
+            then spam
+            else other
+          else
+            spam
+    | [] => spam
+
+
+
+
+noncomputable
+def Pairing_fStrat [Inhabited α] [DecidableEq α] [Fintype α] {win_sets : Finset (Finset α)} (pairing : win_sets → (α × α)):
+  (Positional_Game_World win_sets).fStrategy :=
+  fun hist T leg =>
+    ⟨ Pairing_StratCore win_sets pairing hist leg,
+      (by
+       dsimp [Positional_Game_World]
+       split_ifs with N
+       cases' hist with last L
+       · dsimp [Pairing_StratCore]
+         rw [dif_pos (by decide)]
+         apply List.not_mem_nil
+       · dsimp [Pairing_StratCore]
+         by_cases hxf : ∃ w : win_sets, last = (pairing w).1
+         · rw [dif_pos hxf]
+           split_ifs with M
+           · have := Classical.choose_spec (Pairing_StratCore.proof_1 win_sets (last :: L) leg (T))
+             dsimp [Positional_Game_World] at this
+             rw [if_pos N] at this
+             exact this
+           · have := Classical.choose_spec (Pairing_StratCore.proof_1 win_sets (last :: L) leg (T))
+             dsimp [Positional_Game_World] at this
+             rw [if_pos N] at this
+             exact this
+           · exact M
+         · rw [dif_neg hxf]
+           by_cases hxs : ∃ w : win_sets, last = (pairing w).2
+           · rw [dif_pos hxs]
+             split_ifs with M
+             · have := Classical.choose_spec (Pairing_StratCore.proof_1 win_sets (last :: L) leg (T))
+               dsimp [Positional_Game_World] at this
+               rw [if_pos N] at this
+               exact this
+             · have := Classical.choose_spec (Pairing_StratCore.proof_1 win_sets (last :: L) leg (T))
+               dsimp [Positional_Game_World] at this
+               rw [if_pos N] at this
+               exact this
+             · exact M
+           · rw [dif_neg hxs]
+             split_ifs with M
+             · have := Classical.choose_spec (Pairing_StratCore.proof_1 win_sets (last :: L) leg (T))
+               dsimp [Positional_Game_World] at this
+               rw [if_pos N] at this
+               exact this
+             · have := Classical.choose_spec (Pairing_StratCore.proof_1 win_sets (last :: L) leg (T))
+               dsimp [Positional_Game_World] at this
+               rw [if_pos N] at this
+               exact this
+       )
+      ⟩
+
+
+noncomputable
+def Pairing_sStrat [Inhabited α] [DecidableEq α] [Fintype α] (win_sets : Finset (Finset α)) (pairing : win_sets → (α × α)) :
+  (Positional_Game_World win_sets).sStrategy  :=
+  fun hist T leg =>
+    ⟨ Pairing_StratCore win_sets pairing hist leg,
+      (by
+       dsimp [Positional_Game_World]
+       split_ifs with N
+       cases' hist with last L
+       · dsimp [Pairing_StratCore]
+         rw [dif_pos (by decide)]
+         apply List.not_mem_nil
+       · dsimp [Pairing_StratCore]
+         by_cases hxf : ∃ w : win_sets, last = (pairing w).1
+         · rw [dif_pos hxf]
+           split_ifs with M
+           · have := Classical.choose_spec (Pairing_StratCore.proof_2 win_sets (last :: L) leg (T))
+             dsimp [Positional_Game_World] at this
+             rw [if_pos N] at this
+             exact this
+           · have := Classical.choose_spec (Pairing_StratCore.proof_2 win_sets (last :: L) leg (T))
+             dsimp [Positional_Game_World] at this
+             rw [if_pos N] at this
+             exact this
+           · exact M
+         · rw [dif_neg hxf]
+           by_cases hxs : ∃ w : win_sets, last = (pairing w).2
+           · rw [dif_pos hxs]
+             split_ifs with M
+             · have := Classical.choose_spec (Pairing_StratCore.proof_2 win_sets (last :: L) leg (T))
+               dsimp [Positional_Game_World] at this
+               rw [if_pos N] at this
+               exact this
+             · have := Classical.choose_spec (Pairing_StratCore.proof_2 win_sets (last :: L) leg (T))
+               dsimp [Positional_Game_World] at this
+               rw [if_pos N] at this
+               exact this
+             · exact M
+           · rw [dif_neg hxs]
+             split_ifs with M
+             · have := Classical.choose_spec (Pairing_StratCore.proof_2 win_sets (last :: L) leg (T))
+               dsimp [Positional_Game_World] at this
+               rw [if_pos N] at this
+               exact this
+             · have := Classical.choose_spec (Pairing_StratCore.proof_2 win_sets (last :: L) leg (T))
+               dsimp [Positional_Game_World] at this
+               rw [if_pos N] at this
+               exact this
+       )
+      ⟩
+
+
+
+lemma Positional_Game_World.fst_colored_suffix [Inhabited α] [DecidableEq α] [Fintype α] {win_sets : Finset (Finset α)}
+  (h H : List α) (su : h <:+ H) (leg : (Positional_Game_World win_sets).hist_legal H)
+  (x : α) (main : (State_from_history (Positional_Game_World win_sets).init_game_state (Positional_Game_World win_sets).fst_transition (Positional_Game_World win_sets).snd_transition h) x = 1) :
+  (State_from_history (Positional_Game_World win_sets).init_game_state (Positional_Game_World win_sets).fst_transition (Positional_Game_World win_sets).snd_transition H) x = 1 :=
+  by
+  induction' H with X H ih
+  · rw [List.suffix_nil] at su
+    rw [su] at main
+    exact main
+  · rw [List.suffix_cons_iff] at su
+    cases' su with su su
+    · rw [su] at main
+      exact main
+    · cases' leg
+      rename_i sofar _
+      specialize ih su sofar
+      dsimp [State_from_history, Positional_Game_World]
+      rw [ite_self]
+      cases' H with Y H
+      · exfalso
+        dsimp [State_from_history, Positional_Game_World] at ih
+        contradiction
+      · dsimp [State_from_history, Positional_Game_World] at ih
+        rw [ite_self] at ih
+        dsimp [PosGame_trans] at *
+        split_ifs at ih with mem T
+        · rw [if_pos (by apply List.mem_cons_of_mem ; exact mem )]
+          rw [List.reverse_cons]
+          rw [if_pos (by rw [← List.mem_reverse] at mem ; rw [List.indexOf_append_of_mem mem] ; exact T)]
+        · contradiction
+        · contradiction
+
+lemma Positional_Game_World.snd_colored_suffix [Inhabited α] [DecidableEq α] [Fintype α] {win_sets : Finset (Finset α)}
+  (h H : List α) (su : h <:+ H) (leg : (Positional_Game_World win_sets).hist_legal H)
+  (x : α) (main : (State_from_history (Positional_Game_World win_sets).init_game_state (Positional_Game_World win_sets).fst_transition (Positional_Game_World win_sets).snd_transition h) x = 2) :
+  (State_from_history (Positional_Game_World win_sets).init_game_state (Positional_Game_World win_sets).fst_transition (Positional_Game_World win_sets).snd_transition H) x = 2 :=
+  by
+  induction' H with X H ih
+  · rw [List.suffix_nil] at su
+    rw [su] at main
+    exact main
+  · rw [List.suffix_cons_iff] at su
+    cases' su with su su
+    · rw [su] at main
+      exact main
+    · cases' leg
+      rename_i sofar _
+      specialize ih su sofar
+      dsimp [State_from_history, Positional_Game_World]
+      rw [ite_self]
+      cases' H with Y H
+      · exfalso
+        dsimp [State_from_history, Positional_Game_World] at ih
+        contradiction
+      · dsimp [State_from_history, Positional_Game_World] at ih
+        rw [ite_self] at ih
+        dsimp [PosGame_trans] at *
+        split_ifs at ih with mem T
+        · contradiction
+        · rw [if_pos (by apply List.mem_cons_of_mem ; exact mem )]
+          rw [List.reverse_cons]
+          rw [if_neg (by rw [← List.mem_reverse] at mem ; rw [List.indexOf_append_of_mem mem] ; exact T)]
+        · contradiction
+
+
+
+
+private def colored [Inhabited α] [DecidableEq α] [Fintype α] {win_sets : Finset (Finset α)} (pairing : win_sets → (α × α))
+  (f_strat : (Positional_Game_World win_sets).fStrategy)
+  (pair : α × α) :=
+  {m : Nat |
+    let S := (State_from_history (Positional_Game_World win_sets).init_game_state (Positional_Game_World win_sets).fst_transition (Positional_Game_World win_sets).snd_transition ((Positional_Game_World win_sets).hist_on_turn f_strat (Pairing_sStrat win_sets pairing) m).val) ;
+    S pair.1 ≠ 0 ∨ S pair.2 ≠ 0}
+
+private lemma colored_nonempty [Inhabited α] [DecidableEq α] [Fintype α] {win_sets : Finset (Finset α)} {pairing : win_sets → (α × α)}
+  (hg : Pairing_condition win_sets pairing) {n : Nat}
+  (f_strat : (Positional_Game_World win_sets).fStrategy)
+  (H : List α) (Hsuf : H <:+ ((Positional_Game_World win_sets).hist_on_turn f_strat (Pairing_sStrat win_sets pairing) (n+1)).val )
+  (W : Finset α) (W_win : W ∈ win_sets) (W_sub : W ⊆ Finset.filter (fun x => State_from_history (fun _ => (0 : Fin 3)) (fun hist act => PosGame_trans (act :: hist)) (fun hist act => PosGame_trans (act :: hist)) H x = 1) Finset.univ)
+   :
+  Set.Nonempty (colored pairing f_strat (pairing ⟨W, W_win⟩)) :=
+  by
+  use (n+1)
+  have mem_fst := W_sub (hg.has_pairing ⟨W, W_win⟩).mem_fst
+  rw [Finset.mem_filter] at mem_fst
+  have := Positional_Game_World.fst_colored_suffix H
+            ((Positional_Game_World win_sets).hist_on_turn f_strat (Pairing_sStrat win_sets pairing) (n+1)).val
+            Hsuf
+            ((Positional_Game_World win_sets).hist_on_turn f_strat (Pairing_sStrat win_sets pairing) (n+1)).prop.1
+            (pairing ⟨W, W_win⟩).1 (mem_fst.2)
+  dsimp [colored]
+  left
+  rw [this]
+  decide
+
+private lemma first_colored_turn_neq_zero [Inhabited α] [DecidableEq α] [Fintype α] {win_sets : Finset (Finset α)} {pairing : win_sets → (α × α)}
+  (hg : Pairing_condition win_sets pairing) {n : Nat}
+  (f_strat : (Positional_Game_World win_sets).fStrategy)
+  (H : List α) (Hsuf : H <:+ ((Positional_Game_World win_sets).hist_on_turn f_strat (Pairing_sStrat win_sets pairing) (n+1)).val )
+  (W : Finset α) (W_win : W ∈ win_sets) (W_sub : W ⊆ Finset.filter (fun x => State_from_history (fun _ => 0) (fun hist act => PosGame_trans (act :: hist)) (fun hist act => PosGame_trans (act :: hist)) H x = 1) Finset.univ) :
+  WellFounded.min Nat.lt_wfRel.wf (colored pairing f_strat (pairing ⟨W, W_win⟩)) (colored_nonempty hg f_strat H Hsuf W W_win W_sub) ≠ 0 :=
+  by
+  intro con
+  have M_mem := WellFounded.min_mem Nat.lt_wfRel.wf (colored pairing f_strat (pairing ⟨W, W_win⟩)) (colored_nonempty hg f_strat H Hsuf W W_win W_sub)
+  rw [con] at M_mem
+  dsimp [colored] at M_mem
+  dsimp [Game_World_wDraw.hist_on_turn, Game_World.hist_on_turn, State_from_history, Positional_Game_World] at M_mem
+  rw [or_self] at M_mem
+  contradiction
+
+
+
+
+lemma Nat.succ_of_ne_zero {n : Nat} (h : n ≠ 0) : ∃ m, n = m+1 := by
+  cases' n with n
+  · contradiction
+  · use n
+
+
+lemma List.eq_of_mem_cons_not_mem {l : List α} {x y : α} (h1 : y ∉ l) (h2 : y ∈  x :: l) : y = x := by
+  simp_all only [mem_cons, or_false]
+
+private lemma second_uncolored [Inhabited α] [DecidableEq α] [Fintype α] {win_sets : Finset (Finset α)} {pairing : win_sets → (α × α)}
+  (hg : Pairing_condition win_sets pairing) {n : Nat}
+  (f_strat : (Positional_Game_World win_sets).fStrategy)
+  (H : List α) (Hsuf : H <:+ ((Positional_Game_World win_sets).hist_on_turn f_strat (Pairing_sStrat win_sets pairing) (n+1)).val )
+  (W : Finset α) (W_win : W ∈ win_sets) (W_sub : W ⊆ Finset.filter (fun x => State_from_history (fun _ => 0) (fun hist act => PosGame_trans (act :: hist)) (fun hist act => PosGame_trans (act :: hist)) H x = 1) Finset.univ)
+  : let M := WellFounded.min Nat.lt_wfRel.wf (colored pairing f_strat (pairing ⟨W, W_win⟩)) (colored_nonempty hg f_strat H Hsuf W W_win W_sub)
+  let Hi :=  (((Positional_Game_World win_sets).hist_on_turn f_strat (Pairing_sStrat win_sets pairing)))
+  (State_from_history (Positional_Game_World win_sets).toGame_World.init_game_state
+      (Positional_Game_World win_sets).toGame_World.fst_transition
+      (Positional_Game_World win_sets).toGame_World.snd_transition
+      (Hi M) (pairing ⟨W, W_win⟩).1 ≠ 0) →
+  (State_from_history (Positional_Game_World win_sets).toGame_World.init_game_state
+      (Positional_Game_World win_sets).toGame_World.fst_transition
+      (Positional_Game_World win_sets).toGame_World.snd_transition
+      (Hi M) (pairing ⟨W, W_win⟩).2 = 0) :=
+  by
+  intro M Hi M_mem
+  by_contra con
+  replace con := Positional_Game_World_mem_state' win_sets (pairing ⟨W, W_win⟩).2  _ con
+  by_cases Q : M = 0
+  · exact (first_colored_turn_neq_zero hg f_strat H Hsuf W W_win W_sub) Q
+  · obtain ⟨m,mdef⟩ := Nat.succ_of_ne_zero Q
+    rw [mdef] at con
+    have : m ∉ (colored pairing f_strat (pairing ⟨W, W_win⟩)) :=
+      by
+      intro con
+      apply WellFounded.not_lt_min Nat.lt_wfRel.wf (colored pairing f_strat (pairing ⟨W, W_win⟩)) (colored_nonempty hg f_strat H Hsuf W W_win W_sub) con
+      dsimp [M] at mdef
+      rw [mdef]
+      apply Nat.lt_succ_self
+    dsimp [colored] at this
+    have that : (pairing ⟨W, W_win⟩).1 ∈ (Hi (M)).val :=
+      by
+      apply Positional_Game_World_mem_state' win_sets
+      exact M_mem
+    rw [mdef] at that
+    simp_rw [← not_and_or, not_not] at this
+    have nm1 : (pairing ⟨W, W_win⟩).1 ∉ (Hi m).val :=
+      by
+      intro con
+      exact (Positional_Game_World_mem_state win_sets _ _ con) this.1
+    have nm2 : (pairing ⟨W, W_win⟩).2 ∉ (Hi m).val :=
+      by
+      intro con
+      exact (Positional_Game_World_mem_state win_sets _ _ con) this.2
+    by_cases T : Turn_fst (m+1)
+    · dsimp [Hi, Game_World_wDraw.hist_on_turn, Game_World.hist_on_turn] at that con
+      rw [dif_pos T] at that con
+      replace nm1 := List.eq_of_mem_cons_not_mem nm1 that
+      replace nm2 := List.eq_of_mem_cons_not_mem nm2 con
+      apply (hg.has_pairing ⟨W, W_win⟩).dif
+      rw [nm1,nm2]
+    · dsimp [Hi, Game_World_wDraw.hist_on_turn, Game_World.hist_on_turn] at that con
+      rw [dif_neg T] at that con
+      replace nm1 := List.eq_of_mem_cons_not_mem nm1 that
+      replace nm2 := List.eq_of_mem_cons_not_mem nm2 con
+      apply (hg.has_pairing ⟨W, W_win⟩).dif
+      rw [nm1,nm2]
+
+
+private lemma first_uncolored [Inhabited α] [DecidableEq α] [Fintype α] {win_sets : Finset (Finset α)} {pairing : win_sets → (α × α)}
+  (hg : Pairing_condition win_sets pairing) {n : Nat}
+  (f_strat : (Positional_Game_World win_sets).fStrategy)
+  (H : List α) (Hsuf : H <:+ ((Positional_Game_World win_sets).hist_on_turn f_strat (Pairing_sStrat win_sets pairing) (n+1)).val )
+  (W : Finset α) (W_win : W ∈ win_sets) (W_sub : W ⊆ Finset.filter (fun x => State_from_history (fun _ => 0) (fun hist act => PosGame_trans (act :: hist)) (fun hist act => PosGame_trans (act :: hist)) H x = 1) Finset.univ)
+  : let M := WellFounded.min Nat.lt_wfRel.wf (colored pairing f_strat (pairing ⟨W, W_win⟩)) (colored_nonempty hg f_strat H Hsuf W W_win W_sub)
+  let Hi :=  (((Positional_Game_World win_sets).hist_on_turn f_strat (Pairing_sStrat win_sets pairing)))
+  (State_from_history (Positional_Game_World win_sets).toGame_World.init_game_state
+      (Positional_Game_World win_sets).toGame_World.fst_transition
+      (Positional_Game_World win_sets).toGame_World.snd_transition
+      (Hi M) (pairing ⟨W, W_win⟩).2 ≠ 0) →
+  (State_from_history (Positional_Game_World win_sets).toGame_World.init_game_state
+      (Positional_Game_World win_sets).toGame_World.fst_transition
+      (Positional_Game_World win_sets).toGame_World.snd_transition
+      (Hi M) (pairing ⟨W, W_win⟩).1 = 0) :=
+  by
+  intro M Hi M_mem
+  by_contra con
+  replace con := Positional_Game_World_mem_state' win_sets (pairing ⟨W, W_win⟩).1  _ con
+  by_cases Q : M = 0
+  · exact (first_colored_turn_neq_zero hg f_strat H Hsuf W W_win W_sub) Q
+  · obtain ⟨m,mdef⟩ := Nat.succ_of_ne_zero Q
+    rw [mdef] at con
+    have : m ∉ (colored pairing f_strat (pairing ⟨W, W_win⟩)) :=
+      by
+      intro con
+      apply WellFounded.not_lt_min Nat.lt_wfRel.wf (colored pairing f_strat (pairing ⟨W, W_win⟩)) (colored_nonempty hg f_strat H Hsuf W W_win W_sub) con
+      dsimp [M] at mdef
+      rw [mdef]
+      apply Nat.lt_succ_self
+    dsimp [colored] at this
+    have that : (pairing ⟨W, W_win⟩).2 ∈ (Hi (M)).val :=
+      by
+      apply Positional_Game_World_mem_state' win_sets
+      exact M_mem
+    rw [mdef] at that
+    simp_rw [← not_and_or, not_not] at this
+    have nm1 : (pairing ⟨W, W_win⟩).1 ∉ (Hi m).val :=
+      by
+      intro con
+      exact (Positional_Game_World_mem_state win_sets _ _ con) this.1
+    have nm2 : (pairing ⟨W, W_win⟩).2 ∉ (Hi m).val :=
+      by
+      intro con
+      exact (Positional_Game_World_mem_state win_sets _ _ con) this.2
+    by_cases T : Turn_fst (m+1)
+    · dsimp [Hi, Game_World_wDraw.hist_on_turn, Game_World.hist_on_turn] at that con
+      rw [dif_pos T] at that con
+      replace nm2 := List.eq_of_mem_cons_not_mem nm2 that
+      replace nm1 := List.eq_of_mem_cons_not_mem nm1 con
+      apply (hg.has_pairing ⟨W, W_win⟩).dif
+      rw [nm1,nm2]
+    · dsimp [Hi, Game_World_wDraw.hist_on_turn, Game_World.hist_on_turn] at that con
+      rw [dif_neg T] at that con
+      replace nm2 := List.eq_of_mem_cons_not_mem nm2 that
+      replace nm1 := List.eq_of_mem_cons_not_mem nm1 con
+      apply (hg.has_pairing ⟨W, W_win⟩).dif
+      rw [nm1,nm2]
+
+
+
+private lemma color_pairing_at_win [Inhabited α] [DecidableEq α] [Fintype α] {win_sets : Finset (Finset α)} {pairing : win_sets → (α × α)}
+  (hg : Pairing_condition win_sets pairing)
+  (H : List α) (W : Finset α) (W_win : W ∈ win_sets) (W_sub : W ⊆ Finset.filter (fun x => State_from_history (fun _ => 0) (fun hist act => PosGame_trans (act :: hist)) (fun hist act => PosGame_trans (act :: hist)) H x = 1) Finset.univ) :
+  State_from_history (Positional_Game_World win_sets).toGame_World.init_game_state
+    (Positional_Game_World win_sets).toGame_World.fst_transition
+    (Positional_Game_World win_sets).toGame_World.snd_transition H (pairing { val := W, property := W_win }).1 =
+  1 :=
+  by
+  have mem_fst := W_sub (hg.has_pairing ⟨W, W_win⟩).mem_fst
+  rw [Finset.mem_filter] at mem_fst
+  apply mem_fst.2
+
+private lemma first_colored_by_fst [Inhabited α] [DecidableEq α] [Fintype α] {win_sets : Finset (Finset α)} {pairing : win_sets → (α × α)}
+  (hg : Pairing_condition win_sets pairing) {n : Nat}
+  (f_strat : (Positional_Game_World win_sets).fStrategy)
+  (H : List α) (Hsuf : H <:+ ((Positional_Game_World win_sets).hist_on_turn f_strat (Pairing_sStrat win_sets pairing) (n+1)).val )
+  (W : Finset α) (W_win : W ∈ win_sets) (W_sub : W ⊆ Finset.filter (fun x => State_from_history (fun _ => 0) (fun hist act => PosGame_trans (act :: hist)) (fun hist act => PosGame_trans (act :: hist)) H x = 1) Finset.univ)
+  : let M := WellFounded.min Nat.lt_wfRel.wf (colored pairing f_strat (pairing ⟨W, W_win⟩)) (colored_nonempty hg f_strat H Hsuf W W_win W_sub)
+  let Hi :=  (((Positional_Game_World win_sets).hist_on_turn f_strat (Pairing_sStrat win_sets pairing)))
+  (State_from_history (Positional_Game_World win_sets).toGame_World.init_game_state
+      (Positional_Game_World win_sets).toGame_World.fst_transition
+      (Positional_Game_World win_sets).toGame_World.snd_transition
+      (Hi M) (pairing ⟨W, W_win⟩).1 ≠ 0) →
+  (State_from_history (Positional_Game_World win_sets).toGame_World.init_game_state
+      (Positional_Game_World win_sets).toGame_World.fst_transition
+      (Positional_Game_World win_sets).toGame_World.snd_transition
+      (Hi M) (pairing ⟨W, W_win⟩).1 = 1) :=
+  by
+  intro M Hi col
+  by_contra con
+  have bd := Fin.le_val_last (State_from_history (Positional_Game_World win_sets).toGame_World.init_game_state (Positional_Game_World win_sets).toGame_World.fst_transition (Positional_Game_World win_sets).toGame_World.snd_transition (↑(Hi M)) (pairing { val := W, property := W_win }).1)
+  rw [Fin.ne_iff_vne] at col
+  dsimp at col
+  simp_rw [← Nat.one_le_iff_ne_zero, le_iff_eq_or_lt] at col
+  cases' col with col col
+  · simp_rw [Fin.ne_iff_vne] at con
+    apply con col.symm
+  · rw [← Nat.succ_le] at col
+    replace col := le_antisymm bd col
+    -- refactor with colored_nonempty
+    have mem_fst := W_sub (hg.has_pairing ⟨W, W_win⟩).mem_fst
+    rw [Finset.mem_filter] at mem_fst
+    have := Positional_Game_World.fst_colored_suffix H
+            ((Positional_Game_World win_sets).hist_on_turn f_strat (Pairing_sStrat win_sets pairing) (n+1)).val
+            Hsuf
+            ((Positional_Game_World win_sets).hist_on_turn f_strat (Pairing_sStrat win_sets pairing) (n+1)).prop.1
+            (pairing ⟨W, W_win⟩).1 (mem_fst.2)
+    -- refactor to death ↓
+    have refactor_hard : (n+1) ∈ colored pairing f_strat (pairing ⟨W, W_win⟩) :=
+      by
+      have mem_fst := W_sub (hg.has_pairing ⟨W, W_win⟩).mem_fst
+      rw [Finset.mem_filter] at mem_fst
+      have := Positional_Game_World.fst_colored_suffix H
+                ((Positional_Game_World win_sets).hist_on_turn f_strat (Pairing_sStrat win_sets pairing) (n+1)).val
+                Hsuf
+                ((Positional_Game_World win_sets).hist_on_turn f_strat (Pairing_sStrat win_sets pairing) (n+1)).prop.1
+                (pairing ⟨W, W_win⟩).1 (mem_fst.2)
+      dsimp [colored]
+      left
+      rw [this]
+      decide
+    have M_le := WellFounded.min_le Nat.lt_wfRel.wf refactor_hard (colored_nonempty hg f_strat H Hsuf W W_win W_sub)
+    have almost := Game_World.hist_on_turn_suffix (Positional_Game_World win_sets).toGame_World f_strat (Pairing_sStrat win_sets pairing) _ _ M_le
+    have the := Positional_Game_World.snd_colored_suffix _ _ almost
+        ((Positional_Game_World win_sets).hist_on_turn f_strat (Pairing_sStrat win_sets pairing) (n+1)).prop.1
+        _ col
+    have re := Positional_Game_World.fst_colored_suffix _ _ Hsuf
+        ((Positional_Game_World win_sets).hist_on_turn f_strat (Pairing_sStrat win_sets pairing) (n+1)).prop.1
+        (pairing ⟨W, W_win⟩).1 (color_pairing_at_win hg H W W_win W_sub)
+    rw [Game_World_wDraw.hist_on_turn , the] at re
+    contradiction
+
+
+
+
+
+private lemma color_pairing_at_win_2 [Inhabited α] [DecidableEq α] [Fintype α] {win_sets : Finset (Finset α)} {pairing : win_sets → (α × α)}
+  (hg : Pairing_condition win_sets pairing)
+  (H : List α) (W : Finset α) (W_win : W ∈ win_sets) (W_sub : W ⊆ Finset.filter (fun x => State_from_history (fun _ => 0) (fun hist act => PosGame_trans (act :: hist)) (fun hist act => PosGame_trans (act :: hist)) H x = 1) Finset.univ) :
+  State_from_history (Positional_Game_World win_sets).toGame_World.init_game_state
+    (Positional_Game_World win_sets).toGame_World.fst_transition
+    (Positional_Game_World win_sets).toGame_World.snd_transition H (pairing { val := W, property := W_win }).2 =
+  1 :=
+  by
+  have mem_fst := W_sub (hg.has_pairing ⟨W, W_win⟩).mem_snd
+  rw [Finset.mem_filter] at mem_fst
+  apply mem_fst.2
+
+private lemma second_colored_by_fst [Inhabited α] [DecidableEq α] [Fintype α] {win_sets : Finset (Finset α)} {pairing : win_sets → (α × α)}
+  (hg : Pairing_condition win_sets pairing) {n : Nat}
+  (f_strat : (Positional_Game_World win_sets).fStrategy)
+  (H : List α) (Hsuf : H <:+ ((Positional_Game_World win_sets).hist_on_turn f_strat (Pairing_sStrat win_sets pairing) (n+1)).val )
+  (W : Finset α) (W_win : W ∈ win_sets) (W_sub : W ⊆ Finset.filter (fun x => State_from_history (fun _ => 0) (fun hist act => PosGame_trans (act :: hist)) (fun hist act => PosGame_trans (act :: hist)) H x = 1) Finset.univ)
+  : let M := WellFounded.min Nat.lt_wfRel.wf (colored pairing f_strat (pairing ⟨W, W_win⟩)) (colored_nonempty hg f_strat H Hsuf W W_win W_sub)
+  let Hi :=  (((Positional_Game_World win_sets).hist_on_turn f_strat (Pairing_sStrat win_sets pairing)))
+  (State_from_history (Positional_Game_World win_sets).toGame_World.init_game_state
+      (Positional_Game_World win_sets).toGame_World.fst_transition
+      (Positional_Game_World win_sets).toGame_World.snd_transition
+      (Hi M) (pairing ⟨W, W_win⟩).2 ≠ 0) →
+  (State_from_history (Positional_Game_World win_sets).toGame_World.init_game_state
+      (Positional_Game_World win_sets).toGame_World.fst_transition
+      (Positional_Game_World win_sets).toGame_World.snd_transition
+      (Hi M) (pairing ⟨W, W_win⟩).2 = 1) :=
+  by
+  intro M Hi col
+  by_contra con
+  have bd := Fin.le_val_last (State_from_history (Positional_Game_World win_sets).toGame_World.init_game_state (Positional_Game_World win_sets).toGame_World.fst_transition (Positional_Game_World win_sets).toGame_World.snd_transition (↑(Hi M)) (pairing { val := W, property := W_win }).2)
+  rw [Fin.ne_iff_vne] at col
+  dsimp at col
+  simp_rw [← Nat.one_le_iff_ne_zero, le_iff_eq_or_lt] at col
+  cases' col with col col
+  · simp_rw [Fin.ne_iff_vne] at con
+    apply con col.symm
+  · rw [← Nat.succ_le] at col
+    replace col := le_antisymm bd col
+    -- refactor with colored_nonempty
+    have mem_fst := W_sub (hg.has_pairing ⟨W, W_win⟩).mem_fst
+    rw [Finset.mem_filter] at mem_fst
+    have := Positional_Game_World.fst_colored_suffix H
+            ((Positional_Game_World win_sets).hist_on_turn f_strat (Pairing_sStrat win_sets pairing) (n+1)).val
+            Hsuf
+            ((Positional_Game_World win_sets).hist_on_turn f_strat (Pairing_sStrat win_sets pairing) (n+1)).prop.1
+            (pairing ⟨W, W_win⟩).1 (mem_fst.2)
+    -- refactor to death ↓
+    have refactor_hard : (n+1) ∈ colored pairing f_strat (pairing ⟨W, W_win⟩) :=
+      by
+      have mem_fst := W_sub (hg.has_pairing ⟨W, W_win⟩).mem_fst
+      rw [Finset.mem_filter] at mem_fst
+      have := Positional_Game_World.fst_colored_suffix H
+                ((Positional_Game_World win_sets).hist_on_turn f_strat (Pairing_sStrat win_sets pairing) (n+1)).val
+                Hsuf
+                ((Positional_Game_World win_sets).hist_on_turn f_strat (Pairing_sStrat win_sets pairing) (n+1)).prop.1
+                (pairing ⟨W, W_win⟩).1 (mem_fst.2)
+      dsimp [colored]
+      left
+      rw [this]
+      decide
+    have M_le := WellFounded.min_le Nat.lt_wfRel.wf refactor_hard (colored_nonempty hg f_strat H Hsuf W W_win W_sub)
+    have almost := Game_World.hist_on_turn_suffix (Positional_Game_World win_sets).toGame_World f_strat (Pairing_sStrat win_sets pairing) _ _ M_le
+    have the := Positional_Game_World.snd_colored_suffix _ _ almost
+        ((Positional_Game_World win_sets).hist_on_turn f_strat (Pairing_sStrat win_sets pairing) (n+1)).prop.1
+        _ col
+    have re := Positional_Game_World.fst_colored_suffix _ _ Hsuf
+        ((Positional_Game_World win_sets).hist_on_turn f_strat (Pairing_sStrat win_sets pairing) (n+1)).prop.1
+        (pairing ⟨W, W_win⟩).2 (color_pairing_at_win_2 hg H W W_win W_sub)
+    rw [Game_World_wDraw.hist_on_turn , the] at re
+    contradiction
+
+
+-- may be used to refactor ↑s
+lemma help_1 [Inhabited α] [DecidableEq α] [Fintype α] {win_sets : Finset (Finset α)} {pairing : win_sets → (α × α)}
+  (hg : Pairing_condition win_sets pairing) {n : Nat}
+  (f_strat : (Positional_Game_World win_sets).fStrategy)
+  (H : List α) (Hsuf : H <:+ ((Positional_Game_World win_sets).hist_on_turn f_strat (Pairing_sStrat win_sets pairing) (n+1)).val )
+  (W : Finset α) (W_win : W ∈ win_sets) (W_sub : W ⊆ Finset.filter (fun x => State_from_history (fun _ => 0) (fun hist act => PosGame_trans (act :: hist)) (fun hist act => PosGame_trans (act :: hist)) H x = 1) Finset.univ)
+  {m : Nat} (mdef : WellFounded.min Nat.lt_wfRel.wf (colored pairing f_strat (pairing ⟨W, W_win⟩)) (colored_nonempty hg f_strat H Hsuf W W_win W_sub) = m+1)
+  : let M := WellFounded.min Nat.lt_wfRel.wf (colored pairing f_strat (pairing ⟨W, W_win⟩)) (colored_nonempty hg f_strat H Hsuf W W_win W_sub)
+  let Hi :=  (((Positional_Game_World win_sets).hist_on_turn f_strat (Pairing_sStrat win_sets pairing)))
+  (State_from_history (Positional_Game_World win_sets).toGame_World.init_game_state
+      (Positional_Game_World win_sets).toGame_World.fst_transition
+      (Positional_Game_World win_sets).toGame_World.snd_transition
+      (Hi M) (pairing ⟨W, W_win⟩).1 ≠ 0) →
+  (T : Turn_fst (m+1) ) → f_strat (Hi m).val (by simp_rw [Game_World_wDraw.hist_on_turn, Game_World.hist_on_turn_length] ; exact T) (Hi m).prop.1 = (pairing ⟨W, W_win⟩).1 :=
+  by
+  intro M Hi S T
+  have : m ∉ (colored pairing f_strat (pairing ⟨W, W_win⟩)) :=
+      by
+      intro con
+      apply WellFounded.not_lt_min Nat.lt_wfRel.wf (colored pairing f_strat (pairing ⟨W, W_win⟩)) (colored_nonempty hg f_strat H Hsuf W W_win W_sub) con
+      rw [mdef]
+      apply Nat.lt_succ_self
+  dsimp [colored] at this
+  have that : (pairing ⟨W, W_win⟩).1 ∈ (Hi (M)).val :=
+    by
+    apply Positional_Game_World_mem_state' win_sets
+    exact S
+  dsimp [M] at that
+  rw [mdef] at that
+  simp_rw [← not_and_or, not_not] at this
+  have nm1 : (pairing ⟨W, W_win⟩).1 ∉ (Hi m).val :=
+    by
+    intro con
+    exact (Positional_Game_World_mem_state win_sets _ _ con) this.1
+  dsimp [Game_World_wDraw.hist_on_turn, Game_World.hist_on_turn] at that
+  rw [dif_pos T] at that
+  replace nm1 := List.eq_of_mem_cons_not_mem nm1 that
+  exact nm1.symm
+
+
+
+
+lemma classical_help_1 [Inhabited α] [DecidableEq α] [Fintype α] {win_sets : Finset (Finset α)} {pairing : win_sets → (α × α)}
+  (hg : Pairing_condition win_sets pairing) (W : Finset α) (W_win : W ∈ win_sets) :
+  (hxf : ∃ w : win_sets, (pairing ⟨W,W_win⟩).1 = (pairing w).1) → (pairing (Classical.choose hxf)).2 = (pairing ⟨W,W_win⟩).2 :=
+  by
+  intro hxf
+  have : Classical.choose hxf = ⟨W,W_win⟩ :=
+    by
+    by_contra con
+    apply (hg.pairing_dif ( Classical.choose hxf) ⟨W,W_win⟩ con).strait_fst
+    apply (Classical.choose_spec hxf).symm
+  rw [this]
+
+
+lemma classical_help_2 [Inhabited α] [DecidableEq α] [Fintype α] {win_sets : Finset (Finset α)} {pairing : win_sets → (α × α)}
+  (hg : Pairing_condition win_sets pairing) (W : Finset α) (W_win : W ∈ win_sets) :
+  (hxf : ∃ w : win_sets, (pairing ⟨W,W_win⟩).2 = (pairing w).2) → (pairing (Classical.choose hxf)).1 = (pairing ⟨W,W_win⟩).1 :=
+  by
+  intro hxf
+  have : Classical.choose hxf = ⟨W,W_win⟩ :=
+    by
+    by_contra con
+    apply (hg.pairing_dif ( Classical.choose hxf) ⟨W,W_win⟩ con).strait_snd
+    apply (Classical.choose_spec hxf).symm
+  rw [this]
+
+
+lemma Positional_Game_World.nonzero_colored_suffix [Inhabited α] [DecidableEq α] [Fintype α] {win_sets : Finset (Finset α)}
+  (h H : List α) (su : h <:+ H) (leg : (Positional_Game_World win_sets).hist_legal H)
+  (x : α) (main : (State_from_history (Positional_Game_World win_sets).init_game_state (Positional_Game_World win_sets).fst_transition (Positional_Game_World win_sets).snd_transition h) x ≠ 0) :
+  (State_from_history (Positional_Game_World win_sets).init_game_state (Positional_Game_World win_sets).fst_transition (Positional_Game_World win_sets).snd_transition H) x ≠ 0 :=
+  by
+  have bd := Fin.le_val_last ((State_from_history (Positional_Game_World win_sets).init_game_state (Positional_Game_World win_sets).fst_transition (Positional_Game_World win_sets).snd_transition h) x)
+  rw [Fin.ne_iff_vne] at *
+  dsimp at main
+  simp_rw [← Nat.one_le_iff_ne_zero, le_iff_eq_or_lt] at main
+  cases' main with main main
+  · have := Positional_Game_World.fst_colored_suffix _ _ su leg x (by rw [Fin.eq_iff_veq] ; apply main.symm)
+    rw [this]
+    decide
+  · rw [← Nat.succ_le] at main
+    replace main := le_antisymm bd main
+    have := Positional_Game_World.snd_colored_suffix _ _ su leg x (main)
+    rw [Fin.eq_iff_veq] at main
+    dsimp at main
+    dsimp
+    simp_rw [this]
+    decide
+
+
+private lemma help_2 [Inhabited α] [DecidableEq α] [Fintype α] {win_sets : Finset (Finset α)} {pairing : win_sets → (α × α)}
+  (hg : Pairing_condition win_sets pairing) {n : Nat}
+  (f_strat : (Positional_Game_World win_sets).fStrategy)
+  (H : List α) (Hsuf : H <:+ ((Positional_Game_World win_sets).hist_on_turn f_strat (Pairing_sStrat win_sets pairing) (n+1)).val )
+  (W : Finset α) (W_win : W ∈ win_sets) (W_sub : W ⊆ Finset.filter (fun x => State_from_history (fun _ => 0) (fun hist act => PosGame_trans (act :: hist)) (fun hist act => PosGame_trans (act :: hist)) H x = 1) Finset.univ)
+  {m : Nat} (mdef : WellFounded.min Nat.lt_wfRel.wf (colored pairing f_strat (pairing ⟨W, W_win⟩)) (colored_nonempty hg f_strat H Hsuf W W_win W_sub) = m+1)
+  : let M := WellFounded.min Nat.lt_wfRel.wf (colored pairing f_strat (pairing ⟨W, W_win⟩)) (colored_nonempty hg f_strat H Hsuf W W_win W_sub)
+  let Hi :=  (((Positional_Game_World win_sets).hist_on_turn f_strat (Pairing_sStrat win_sets pairing)))
+  (State_from_history (Positional_Game_World win_sets).toGame_World.init_game_state
+      (Positional_Game_World win_sets).toGame_World.fst_transition
+      (Positional_Game_World win_sets).toGame_World.snd_transition
+      (Hi M) (pairing ⟨W, W_win⟩).1 ≠ 0) →
+  (pairing ⟨W, W_win⟩).2 ∉
+    ((Positional_Game_World win_sets).hist_on_turn f_strat (Pairing_sStrat win_sets pairing) m).val :=
+  by
+  intro M Hi hit con
+  replace con := Positional_Game_World_mem_state win_sets _ _ con
+  replace hit := second_uncolored hg f_strat  H Hsuf W W_win W_sub hit
+  rw [mdef] at hit
+  have con' := Positional_Game_World.nonzero_colored_suffix
+      ((Positional_Game_World win_sets).hist_on_turn f_strat (Pairing_sStrat win_sets pairing) m).val
+      ((Positional_Game_World win_sets).hist_on_turn f_strat (Pairing_sStrat win_sets pairing) (m+1)).val
+      (by rw [Game_World_wDraw.hist_on_turn] ;  apply Game_World.hist_on_turn_suffix ; exact Nat.le_add_right m 1)
+      ((Positional_Game_World win_sets).hist_on_turn f_strat (Pairing_sStrat win_sets pairing) (m+1)).prop.1
+      _ con
+  exact con' hit
+
+
+
+private lemma help_6 [Inhabited α] [DecidableEq α] [Fintype α] {win_sets : Finset (Finset α)} {pairing : win_sets → (α × α)}
+  (hg : Pairing_condition win_sets pairing) {n : Nat}
+  (f_strat : (Positional_Game_World win_sets).fStrategy)
+  (H : List α) (Hsuf : H <:+ ((Positional_Game_World win_sets).hist_on_turn f_strat (Pairing_sStrat win_sets pairing) (n+1)).val )
+  (W : Finset α) (W_win : W ∈ win_sets) (W_sub : W ⊆ Finset.filter (fun x => State_from_history (fun _ => 0) (fun hist act => PosGame_trans (act :: hist)) (fun hist act => PosGame_trans (act :: hist)) H x = 1) Finset.univ)
+  {m : Nat} (mdef : WellFounded.min Nat.lt_wfRel.wf (colored pairing f_strat (pairing ⟨W, W_win⟩)) (colored_nonempty hg f_strat H Hsuf W W_win W_sub) = m+1)
+  : let M := WellFounded.min Nat.lt_wfRel.wf (colored pairing f_strat (pairing ⟨W, W_win⟩)) (colored_nonempty hg f_strat H Hsuf W W_win W_sub)
+  let Hi :=  (((Positional_Game_World win_sets).hist_on_turn f_strat (Pairing_sStrat win_sets pairing)))
+  (State_from_history (Positional_Game_World win_sets).toGame_World.init_game_state
+      (Positional_Game_World win_sets).toGame_World.fst_transition
+      (Positional_Game_World win_sets).toGame_World.snd_transition
+      (Hi M) (pairing ⟨W, W_win⟩).2 ≠ 0) →
+  (pairing ⟨W, W_win⟩).1 ∉
+    ((Positional_Game_World win_sets).hist_on_turn f_strat (Pairing_sStrat win_sets pairing) m).val :=
+  by
+  intro M Hi hit con
+  replace con := Positional_Game_World_mem_state win_sets _ _ con
+  replace hit := first_uncolored hg f_strat  H Hsuf W W_win W_sub hit
+  rw [mdef] at hit
+  have con' := Positional_Game_World.nonzero_colored_suffix
+      ((Positional_Game_World win_sets).hist_on_turn f_strat (Pairing_sStrat win_sets pairing) m).val
+      ((Positional_Game_World win_sets).hist_on_turn f_strat (Pairing_sStrat win_sets pairing) (m+1)).val
+      (by rw [Game_World_wDraw.hist_on_turn] ;  apply Game_World.hist_on_turn_suffix ; exact Nat.le_add_right m 1)
+      ((Positional_Game_World win_sets).hist_on_turn f_strat (Pairing_sStrat win_sets pairing) (m+1)).prop.1
+      _ con
+  exact con' hit
+
+
+
+lemma help_3 [Inhabited α] [DecidableEq α] [Fintype α] {win_sets : Finset (Finset α)} {pairing : win_sets → (α × α)}
+  (hg : Pairing_condition win_sets pairing) {n : Nat}
+  (f_strat : (Positional_Game_World win_sets).fStrategy)
+  (H : List α) (Hsuf : H <:+ ((Positional_Game_World win_sets).hist_on_turn f_strat (Pairing_sStrat win_sets pairing) (n+1)).val )
+  (W : Finset α) (W_win : W ∈ win_sets) (W_sub : W ⊆ Finset.filter (fun x => State_from_history (fun _ => 0) (fun hist act => PosGame_trans (act :: hist)) (fun hist act => PosGame_trans (act :: hist)) H x = 1) Finset.univ)
+  {m : Nat} (mdef : WellFounded.min Nat.lt_wfRel.wf (colored pairing f_strat (pairing ⟨W, W_win⟩)) (colored_nonempty hg f_strat H Hsuf W W_win W_sub) = m+1)
+  : let M := WellFounded.min Nat.lt_wfRel.wf (colored pairing f_strat (pairing ⟨W, W_win⟩)) (colored_nonempty hg f_strat H Hsuf W W_win W_sub)
+  let Hi :=  (((Positional_Game_World win_sets).hist_on_turn f_strat (Pairing_sStrat win_sets pairing)))
+  (State_from_history (Positional_Game_World win_sets).toGame_World.init_game_state
+      (Positional_Game_World win_sets).toGame_World.fst_transition
+      (Positional_Game_World win_sets).toGame_World.snd_transition
+      (Hi M) (pairing ⟨W, W_win⟩).1 ≠ 0) →
+  (T : ¬ Turn_fst (m+1) ) → (Pairing_sStrat win_sets pairing) (Hi m).val (by simp_rw [Game_World_wDraw.hist_on_turn, Game_World.hist_on_turn_length] ; exact T) (Hi m).prop.1 = (pairing ⟨W, W_win⟩).1 :=
+  by
+  intro M Hi S T
+  have : m ∉ (colored pairing f_strat (pairing ⟨W, W_win⟩)) :=
+      by
+      intro con
+      apply WellFounded.not_lt_min Nat.lt_wfRel.wf (colored pairing f_strat (pairing ⟨W, W_win⟩)) (colored_nonempty hg f_strat H Hsuf W W_win W_sub) con
+      rw [mdef]
+      apply Nat.lt_succ_self
+  dsimp [colored] at this
+  have that : (pairing ⟨W, W_win⟩).1 ∈ (Hi (M)).val :=
+    by
+    apply Positional_Game_World_mem_state' win_sets
+    exact S
+  dsimp [M] at that
+  rw [mdef] at that
+  simp_rw [← not_and_or, not_not] at this
+  have nm1 : (pairing ⟨W, W_win⟩).1 ∉ (Hi m).val :=
+    by
+    intro con
+    exact (Positional_Game_World_mem_state win_sets _ _ con) this.1
+  dsimp [Game_World_wDraw.hist_on_turn, Game_World.hist_on_turn] at that
+  rw [dif_neg T] at that
+  replace nm1 := List.eq_of_mem_cons_not_mem nm1 that
+  exact nm1.symm
+
+
+
+lemma help_4 [Inhabited α] [DecidableEq α] [Fintype α] {win_sets : Finset (Finset α)} {pairing : win_sets → (α × α)}
+  (hg : Pairing_condition win_sets pairing) {n : Nat}
+  (f_strat : (Positional_Game_World win_sets).fStrategy)
+  (H : List α) (Hsuf : H <:+ ((Positional_Game_World win_sets).hist_on_turn f_strat (Pairing_sStrat win_sets pairing) (n+1)).val )
+  (W : Finset α) (W_win : W ∈ win_sets) (W_sub : W ⊆ Finset.filter (fun x => State_from_history (fun _ => 0) (fun hist act => PosGame_trans (act :: hist)) (fun hist act => PosGame_trans (act :: hist)) H x = 1) Finset.univ)
+  {m : Nat} (mdef : WellFounded.min Nat.lt_wfRel.wf (colored pairing f_strat (pairing ⟨W, W_win⟩)) (colored_nonempty hg f_strat H Hsuf W W_win W_sub) = m+1)
+  : let M := WellFounded.min Nat.lt_wfRel.wf (colored pairing f_strat (pairing ⟨W, W_win⟩)) (colored_nonempty hg f_strat H Hsuf W W_win W_sub)
+  let Hi :=  (((Positional_Game_World win_sets).hist_on_turn f_strat (Pairing_sStrat win_sets pairing)))
+  (State_from_history (Positional_Game_World win_sets).toGame_World.init_game_state
+      (Positional_Game_World win_sets).toGame_World.fst_transition
+      (Positional_Game_World win_sets).toGame_World.snd_transition
+      (Hi M) (pairing ⟨W, W_win⟩).2 ≠ 0) →
+  (T : Turn_fst (m+1) )→ f_strat (Hi m).val (by simp_rw [Game_World_wDraw.hist_on_turn, Game_World.hist_on_turn_length] ; exact T) (Hi m).prop.1 = (pairing ⟨W, W_win⟩).2 :=
+  by
+  intro M Hi S T
+  have : m ∉ (colored pairing f_strat (pairing ⟨W, W_win⟩)) :=
+      by
+      intro con
+      apply WellFounded.not_lt_min Nat.lt_wfRel.wf (colored pairing f_strat (pairing ⟨W, W_win⟩)) (colored_nonempty hg f_strat H Hsuf W W_win W_sub) con
+      rw [mdef]
+      apply Nat.lt_succ_self
+  dsimp [colored] at this
+  have that : (pairing ⟨W, W_win⟩).2 ∈ (Hi (M)).val :=
+    by
+    apply Positional_Game_World_mem_state' win_sets
+    exact S
+  dsimp [M] at that
+  rw [mdef] at that
+  simp_rw [← not_and_or, not_not] at this
+  have nm1 : (pairing ⟨W, W_win⟩).2 ∉ (Hi m).val :=
+    by
+    intro con
+    exact (Positional_Game_World_mem_state win_sets _ _ con) this.2
+  dsimp [Game_World_wDraw.hist_on_turn, Game_World.hist_on_turn] at that
+  rw [dif_pos T] at that
+  replace nm1 := List.eq_of_mem_cons_not_mem nm1 that
+  exact nm1.symm
+
+
+lemma help_5 [Inhabited α] [DecidableEq α] [Fintype α] {win_sets : Finset (Finset α)} {pairing : win_sets → (α × α)}
+  (hg : Pairing_condition win_sets pairing) {n : Nat}
+  (f_strat : (Positional_Game_World win_sets).fStrategy)
+  (H : List α) (Hsuf : H <:+ ((Positional_Game_World win_sets).hist_on_turn f_strat (Pairing_sStrat win_sets pairing) (n+1)).val )
+  (W : Finset α) (W_win : W ∈ win_sets) (W_sub : W ⊆ Finset.filter (fun x => State_from_history (fun _ => 0) (fun hist act => PosGame_trans (act :: hist)) (fun hist act => PosGame_trans (act :: hist)) H x = 1) Finset.univ)
+  {m : Nat} (mdef : WellFounded.min Nat.lt_wfRel.wf (colored pairing f_strat (pairing ⟨W, W_win⟩)) (colored_nonempty hg f_strat H Hsuf W W_win W_sub) = m+1)
+  : let M := WellFounded.min Nat.lt_wfRel.wf (colored pairing f_strat (pairing ⟨W, W_win⟩)) (colored_nonempty hg f_strat H Hsuf W W_win W_sub)
+  let Hi :=  (((Positional_Game_World win_sets).hist_on_turn f_strat (Pairing_sStrat win_sets pairing)))
+  (State_from_history (Positional_Game_World win_sets).toGame_World.init_game_state
+      (Positional_Game_World win_sets).toGame_World.fst_transition
+      (Positional_Game_World win_sets).toGame_World.snd_transition
+      (Hi M) (pairing ⟨W, W_win⟩).2 ≠ 0) →
+  (T : ¬ Turn_fst (m+1) ) → (Pairing_sStrat win_sets pairing) (Hi m).val (by simp_rw [Game_World_wDraw.hist_on_turn, Game_World.hist_on_turn_length] ; exact T) (Hi m).prop.1 = (pairing ⟨W, W_win⟩).2 :=
+  by
+  intro M Hi S T
+  have : m ∉ (colored pairing f_strat (pairing ⟨W, W_win⟩)) :=
+      by
+      intro con
+      apply WellFounded.not_lt_min Nat.lt_wfRel.wf (colored pairing f_strat (pairing ⟨W, W_win⟩)) (colored_nonempty hg f_strat H Hsuf W W_win W_sub) con
+      rw [mdef]
+      apply Nat.lt_succ_self
+  dsimp [colored] at this
+  have that : (pairing ⟨W, W_win⟩).2 ∈ (Hi (M)).val :=
+    by
+    apply Positional_Game_World_mem_state' win_sets
+    exact S
+  dsimp [M] at that
+  rw [mdef] at that
+  simp_rw [← not_and_or, not_not] at this
+  have nm1 : (pairing ⟨W, W_win⟩).2 ∉ (Hi m).val :=
+    by
+    intro con
+    exact (Positional_Game_World_mem_state win_sets _ _ con) this.2
+  dsimp [Game_World_wDraw.hist_on_turn, Game_World.hist_on_turn] at that
+  rw [dif_neg T] at that
+  replace nm1 := List.eq_of_mem_cons_not_mem nm1 that
+  exact nm1.symm
+
+
+
+private lemma Pairing_StratCore_reacts_fst [Inhabited α] [DecidableEq α] [Fintype α] {win_sets : Finset (Finset α)} {pairing : win_sets → (α × α)}
+  (hg : Pairing_condition win_sets pairing) {n : Nat}
+  (f_strat : (Positional_Game_World win_sets).fStrategy)
+  (H : List α) (Hsuf : H <:+ ((Positional_Game_World win_sets).hist_on_turn f_strat (Pairing_sStrat win_sets pairing) (n+1)).val )
+  (W : Finset α) (W_win : W ∈ win_sets) (W_sub : W ⊆ Finset.filter (fun x => State_from_history (fun _ => 0) (fun hist act => PosGame_trans (act :: hist)) (fun hist act => PosGame_trans (act :: hist)) H x = 1) Finset.univ)
+  : let M := WellFounded.min Nat.lt_wfRel.wf (colored pairing f_strat (pairing ⟨W, W_win⟩)) (colored_nonempty hg f_strat H Hsuf W W_win W_sub)
+  let Hi :=  (((Positional_Game_World win_sets).hist_on_turn f_strat (Pairing_sStrat win_sets pairing)))
+  Turn_fst (M) →
+  (State_from_history (Positional_Game_World win_sets).toGame_World.init_game_state
+      (Positional_Game_World win_sets).toGame_World.fst_transition
+      (Positional_Game_World win_sets).toGame_World.snd_transition
+      (Hi M) (pairing ⟨W, W_win⟩).1 ≠ 0) →
+  (Pairing_StratCore win_sets pairing (Hi M).val (Hi M).prop.1) = (pairing ⟨W, W_win⟩).2 :=
+  by
+  intro M Hi T hit
+  by_cases Q : M = 0
+  · exfalso
+    exact (first_colored_turn_neq_zero hg f_strat H Hsuf W W_win W_sub) Q
+  · obtain ⟨m,mdef⟩ := Nat.succ_of_ne_zero Q
+    rw [mdef]
+    rw [mdef] at T
+    dsimp [Game_World_wDraw.hist_on_turn, Game_World.hist_on_turn]
+    rw [dif_pos T]
+    dsimp [Pairing_StratCore]
+    have hxf : ∃ w, f_strat (Hi m).val (by simp_rw [Game_World_wDraw.hist_on_turn, Game_World.hist_on_turn_length] ; exact T) (Hi m).prop.1 = (pairing w).1 :=
+      by use ⟨W, W_win⟩ ; apply help_1 hg f_strat H Hsuf W W_win W_sub mdef hit T
+    rw [dif_pos (by convert hxf)]
+    have fixHist := help_1 hg f_strat H Hsuf W W_win W_sub mdef hit T
+    dsimp [Game_World_wDraw.hist_on_turn] at fixHist
+    rw [if_neg (by simp_rw [fixHist] ; have := classical_help_1 hg W W_win (by rw [ help_1 hg f_strat H Hsuf W W_win W_sub mdef hit T] at hxf ; exact hxf) ; rw [this] ; apply List.not_mem_cons_of_ne_of_not_mem ; rw [ne_comm] ; exact (hg.has_pairing ⟨W,W_win⟩).dif ; apply help_2 hg f_strat H Hsuf W W_win W_sub mdef hit)]
+    rw [ help_1 hg f_strat H Hsuf W W_win W_sub mdef hit T] at hxf
+    convert classical_help_1 hg W W_win hxf
+
+
+
+lemma interesting [Inhabited α] [DecidableEq α] [Fintype α] {win_sets : Finset (Finset α)} {pairing : win_sets → (α × α)}
+  (hg : Pairing_condition win_sets pairing)
+  (main : ∃ w : win_sets, last = (pairing w).2) :
+  ¬ (∃ w : win_sets, last = (pairing w).1) :=
+  by
+  obtain ⟨W,W_win,main⟩ := main
+  push_neg
+  intro w
+  by_cases Q : W = w
+  · rw [Q, ne_comm]
+    apply (hg.has_pairing w).dif
+  · rw [ne_comm]
+    apply (hg.pairing_dif w W (by rw [ne_comm]; exact Q)).cross_fst
+
+
+
+
+private lemma Pairing_StratCore_reacts_snd [Inhabited α] [DecidableEq α] [Fintype α] {win_sets : Finset (Finset α)} {pairing : win_sets → (α × α)}
+  (hg : Pairing_condition win_sets pairing) {n : Nat}
+  (f_strat : (Positional_Game_World win_sets).fStrategy)
+  (H : List α) (Hsuf : H <:+ ((Positional_Game_World win_sets).hist_on_turn f_strat (Pairing_sStrat win_sets pairing) (n+1)).val )
+  (W : Finset α) (W_win : W ∈ win_sets) (W_sub : W ⊆ Finset.filter (fun x => State_from_history (fun _ => 0) (fun hist act => PosGame_trans (act :: hist)) (fun hist act => PosGame_trans (act :: hist)) H x = 1) Finset.univ)
+  : let M := WellFounded.min Nat.lt_wfRel.wf (colored pairing f_strat (pairing ⟨W, W_win⟩)) (colored_nonempty hg f_strat H Hsuf W W_win W_sub)
+  let Hi :=  (((Positional_Game_World win_sets).hist_on_turn f_strat (Pairing_sStrat win_sets pairing)))
+  Turn_fst (M) →
+  (State_from_history (Positional_Game_World win_sets).toGame_World.init_game_state
+      (Positional_Game_World win_sets).toGame_World.fst_transition
+      (Positional_Game_World win_sets).toGame_World.snd_transition
+      (Hi M) (pairing ⟨W, W_win⟩).2 ≠ 0) →
+  (Pairing_StratCore win_sets pairing (Hi M).val (Hi M).prop.1) = (pairing ⟨W, W_win⟩).1 :=
+  by
+  intro M Hi T hit
+  by_cases Q : M = 0
+  · exfalso
+    exact (first_colored_turn_neq_zero hg f_strat H Hsuf W W_win W_sub) Q
+  · obtain ⟨m,mdef⟩ := Nat.succ_of_ne_zero Q
+    rw [mdef]
+    rw [mdef] at T
+    dsimp [Game_World_wDraw.hist_on_turn, Game_World.hist_on_turn]
+    rw [dif_pos T]
+    dsimp [Pairing_StratCore]
+    have hxf : ∃ w, f_strat (Hi m).val (by simp_rw [Game_World_wDraw.hist_on_turn, Game_World.hist_on_turn_length] ; exact T) (Hi m).prop.1 = (pairing w).2 :=
+      by use ⟨W, W_win⟩ ; apply help_4 hg f_strat H Hsuf W W_win W_sub mdef hit T
+    have fixHist := interesting hg hxf
+    have fixHist2 := help_4 hg f_strat H Hsuf W W_win W_sub mdef hit T
+    dsimp [Game_World_wDraw.hist_on_turn] at fixHist fixHist2 hxf
+    rw [dif_neg fixHist]
+    rw [dif_pos hxf]
+    rw [if_neg (by simp_rw [fixHist2] ; have := classical_help_2 hg W W_win (by rw [fixHist2] at hxf ; exact hxf) ; rw [this] ; apply List.not_mem_cons_of_ne_of_not_mem ; rw [ne_comm] ; exact ne_comm.mp (hg.has_pairing ⟨W,W_win⟩).dif ; apply help_6 hg f_strat H Hsuf W W_win W_sub mdef hit)]
+    rw [fixHist2] at hxf
+    convert classical_help_2 hg W W_win hxf
+
+
+
+lemma help_1_3 [Inhabited α] [DecidableEq α] [Fintype α] {win_sets : Finset (Finset α)} {pairing : win_sets → (α × α)}
+  (hg : Pairing_condition win_sets pairing) {n : Nat}
+  (f_strat : (Positional_Game_World win_sets).fStrategy)
+  (H : List α) (Hsuf : H <:+ ((Positional_Game_World win_sets).hist_on_turn f_strat (Pairing_sStrat win_sets pairing) (n+1)).val )
+  (W : Finset α) (W_win : W ∈ win_sets) (W_sub : W ⊆ Finset.filter (fun x => State_from_history (fun _ => 0) (fun hist act => PosGame_trans (act :: hist)) (fun hist act => PosGame_trans (act :: hist)) H x = 1) Finset.univ)
+  {m : Nat} (mdef : WellFounded.min Nat.lt_wfRel.wf (colored pairing f_strat (pairing ⟨W, W_win⟩)) (colored_nonempty hg f_strat H Hsuf W W_win W_sub) = m+1)
+  : let M := WellFounded.min Nat.lt_wfRel.wf (colored pairing f_strat (pairing ⟨W, W_win⟩)) (colored_nonempty hg f_strat H Hsuf W W_win W_sub)
+  let Hi :=  (((Positional_Game_World win_sets).hist_on_turn f_strat (Pairing_sStrat win_sets pairing)))
+  (State_from_history (Positional_Game_World win_sets).toGame_World.init_game_state
+      (Positional_Game_World win_sets).toGame_World.fst_transition
+      (Positional_Game_World win_sets).toGame_World.snd_transition
+      (Hi M) (pairing ⟨W, W_win⟩).1 ≠ 0) →
+  (Hi (M)).val = (pairing ⟨W, W_win⟩).1  :: (Hi (m)).val :=
+  by
+  intro M Hi S
+  by_cases T : Turn_fst (m+1)
+  · dsimp [M]
+    rw [mdef, Game_World_wDraw.hist_on_turn, Game_World.hist_on_turn, dif_pos T]
+    dsimp
+    congr
+    apply help_1 hg f_strat H Hsuf W W_win W_sub mdef S T
+  · dsimp [M]
+    rw [mdef, Game_World_wDraw.hist_on_turn, Game_World.hist_on_turn, dif_neg T]
+    dsimp
+    congr
+    apply help_3 hg f_strat H Hsuf W W_win W_sub mdef S T
+
+
+lemma help_1_3_2 [Inhabited α] [DecidableEq α] [Fintype α] {win_sets : Finset (Finset α)} {pairing : win_sets → (α × α)}
+  (hg : Pairing_condition win_sets pairing) {n : Nat}
+  (f_strat : (Positional_Game_World win_sets).fStrategy)
+  (H : List α) (Hsuf : H <:+ ((Positional_Game_World win_sets).hist_on_turn f_strat (Pairing_sStrat win_sets pairing) (n+1)).val )
+  (W : Finset α) (W_win : W ∈ win_sets) (W_sub : W ⊆ Finset.filter (fun x => State_from_history (fun _ => 0) (fun hist act => PosGame_trans (act :: hist)) (fun hist act => PosGame_trans (act :: hist)) H x = 1) Finset.univ)
+  {m : Nat} (mdef : WellFounded.min Nat.lt_wfRel.wf (colored pairing f_strat (pairing ⟨W, W_win⟩)) (colored_nonempty hg f_strat H Hsuf W W_win W_sub) = m+1)
+  : let M := WellFounded.min Nat.lt_wfRel.wf (colored pairing f_strat (pairing ⟨W, W_win⟩)) (colored_nonempty hg f_strat H Hsuf W W_win W_sub)
+  let Hi :=  (((Positional_Game_World win_sets).hist_on_turn f_strat (Pairing_sStrat win_sets pairing)))
+  (State_from_history (Positional_Game_World win_sets).toGame_World.init_game_state
+      (Positional_Game_World win_sets).toGame_World.fst_transition
+      (Positional_Game_World win_sets).toGame_World.snd_transition
+      (Hi M) (pairing ⟨W, W_win⟩).2 ≠ 0) →
+  (Hi (M)).val = (pairing ⟨W, W_win⟩).2 :: (Hi (m)).val :=
+  by
+  intro M Hi S
+  by_cases T : Turn_fst (m+1)
+  · dsimp [M]
+    rw [mdef, Game_World_wDraw.hist_on_turn, Game_World.hist_on_turn, dif_pos T]
+    dsimp
+    congr
+    apply help_4 hg f_strat H Hsuf W W_win W_sub mdef S T
+  · dsimp [M]
+    rw [mdef, Game_World_wDraw.hist_on_turn, Game_World.hist_on_turn, dif_neg T]
+    dsimp
+    congr
+    apply help_5 hg f_strat H Hsuf W W_win W_sub mdef S T
+
+
+lemma almost [Inhabited α] [DecidableEq α] [Fintype α] {win_sets : Finset (Finset α)} {pairing : win_sets → (α × α)}
+  (hg : Pairing_condition win_sets pairing) {n : Nat}
+  (f_strat : (Positional_Game_World win_sets).fStrategy)
+  (H : List α) (Hsuf : H <:+ ((Positional_Game_World win_sets).hist_on_turn f_strat (Pairing_sStrat win_sets pairing) (n+1)).val )
+  (W : Finset α) (W_win : W ∈ win_sets) (W_sub : W ⊆ Finset.filter (fun x => State_from_history (fun _ => 0) (fun hist act => PosGame_trans (act :: hist)) (fun hist act => PosGame_trans (act :: hist)) H x = 1) Finset.univ)
+  {m : Nat} (mdef : WellFounded.min Nat.lt_wfRel.wf (colored pairing f_strat (pairing ⟨W, W_win⟩)) (colored_nonempty hg f_strat H Hsuf W W_win W_sub) = m+1)
+  : let M := WellFounded.min Nat.lt_wfRel.wf (colored pairing f_strat (pairing ⟨W, W_win⟩)) (colored_nonempty hg f_strat H Hsuf W W_win W_sub)
+  let Hi :=  (((Positional_Game_World win_sets).hist_on_turn f_strat (Pairing_sStrat win_sets pairing)))
+  (State_from_history (Positional_Game_World win_sets).toGame_World.init_game_state
+      (Positional_Game_World win_sets).toGame_World.fst_transition
+      (Positional_Game_World win_sets).toGame_World.snd_transition
+      (Hi M) (pairing ⟨W, W_win⟩).1 ≠ 0) →
+  (State_from_history (Positional_Game_World win_sets).toGame_World.init_game_state
+      (Positional_Game_World win_sets).toGame_World.fst_transition
+      (Positional_Game_World win_sets).toGame_World.snd_transition
+      ((pairing ⟨W, W_win⟩).1  :: (Hi (m)).val)
+      (pairing ⟨W, W_win⟩).1 = 1) :=
+  by
+  intro M Hi S
+  rw [← help_1_3 hg f_strat H Hsuf W W_win W_sub mdef S]
+  apply first_colored_by_fst hg f_strat H Hsuf W W_win W_sub S
+
+
+
+lemma almost2 [Inhabited α] [DecidableEq α] [Fintype α] {win_sets : Finset (Finset α)} {pairing : win_sets → (α × α)}
+  (hg : Pairing_condition win_sets pairing) {n : Nat}
+  (f_strat : (Positional_Game_World win_sets).fStrategy)
+  (H : List α) (Hsuf : H <:+ ((Positional_Game_World win_sets).hist_on_turn f_strat (Pairing_sStrat win_sets pairing) (n+1)).val )
+  (W : Finset α) (W_win : W ∈ win_sets) (W_sub : W ⊆ Finset.filter (fun x => State_from_history (fun _ => 0) (fun hist act => PosGame_trans (act :: hist)) (fun hist act => PosGame_trans (act :: hist)) H x = 1) Finset.univ)
+  {m : Nat} (mdef : WellFounded.min Nat.lt_wfRel.wf (colored pairing f_strat (pairing ⟨W, W_win⟩)) (colored_nonempty hg f_strat H Hsuf W W_win W_sub) = m+1)
+  : let M := WellFounded.min Nat.lt_wfRel.wf (colored pairing f_strat (pairing ⟨W, W_win⟩)) (colored_nonempty hg f_strat H Hsuf W W_win W_sub)
+  let Hi :=  (((Positional_Game_World win_sets).hist_on_turn f_strat (Pairing_sStrat win_sets pairing)))
+  (State_from_history (Positional_Game_World win_sets).toGame_World.init_game_state
+      (Positional_Game_World win_sets).toGame_World.fst_transition
+      (Positional_Game_World win_sets).toGame_World.snd_transition
+      (Hi M) (pairing ⟨W, W_win⟩).2 ≠ 0) →
+  (State_from_history (Positional_Game_World win_sets).toGame_World.init_game_state
+      (Positional_Game_World win_sets).toGame_World.fst_transition
+      (Positional_Game_World win_sets).toGame_World.snd_transition
+      ((pairing ⟨W, W_win⟩).2  :: (Hi (m)).val)
+      (pairing ⟨W, W_win⟩).2 = 1) :=
+  by
+  intro M Hi S
+  rw [← help_1_3_2 hg f_strat H Hsuf W W_win W_sub mdef S]
+  apply second_colored_by_fst hg f_strat H Hsuf W W_win W_sub S
+
+
+
+
+lemma there [Inhabited α] [DecidableEq α] [Fintype α] {win_sets : Finset (Finset α)} {pairing : win_sets → (α × α)}
+  (hg : Pairing_condition win_sets pairing) {n : Nat}
+  (f_strat : (Positional_Game_World win_sets).fStrategy)
+  (Neu : ∀ k ≤ n, Game_World_wDraw.state_on_turn_neutral (Positional_Game_World win_sets) f_strat (Pairing_sStrat win_sets pairing) k)
+  (H : List α) (Hsuf : H <:+ ((Positional_Game_World win_sets).hist_on_turn f_strat (Pairing_sStrat win_sets pairing) (n+1)).val )
+  (W : Finset α) (W_win : W ∈ win_sets) (W_sub : W ⊆ Finset.filter (fun x => State_from_history (fun _ => 0) (fun hist act => PosGame_trans (act :: hist)) (fun hist act => PosGame_trans (act :: hist)) H x = 1) Finset.univ)
+  {m : Nat} (mdef : WellFounded.min Nat.lt_wfRel.wf (colored pairing f_strat (pairing ⟨W, W_win⟩)) (colored_nonempty hg f_strat H Hsuf W W_win W_sub) = m+1)
+  : let M := WellFounded.min Nat.lt_wfRel.wf (colored pairing f_strat (pairing ⟨W, W_win⟩)) (colored_nonempty hg f_strat H Hsuf W W_win W_sub)
+  let Hi :=  (((Positional_Game_World win_sets).hist_on_turn f_strat (Pairing_sStrat win_sets pairing)))
+  (State_from_history (Positional_Game_World win_sets).toGame_World.init_game_state
+      (Positional_Game_World win_sets).toGame_World.fst_transition
+      (Positional_Game_World win_sets).toGame_World.snd_transition
+      (Hi M) (pairing ⟨W, W_win⟩).1 ≠ 0) →
+  Turn_fst M :=
+  by
+  intro M Hi S
+  dsimp [M]
+  rw [mdef]
+  have := Positional_Game_World.turn_fst_of_col_fst (Hi m).val (pairing ⟨W, W_win⟩).1
+    (by have := (Hi M).prop.1 ; rw [help_1_3 hg f_strat H Hsuf W W_win W_sub mdef S] at this ; exact this)
+    (almost hg f_strat H Hsuf W W_win W_sub mdef S)
+    (by rw [← Game_World_wDraw.state_on_turn_neutral_State_from_history_neutral]
+        apply Neu
+        rw [← Nat.succ_le_succ_iff, Nat.succ_eq_add_one, ← mdef]
+        apply  WellFounded.min_le Nat.lt_wfRel.wf _ (colored_nonempty hg f_strat H Hsuf W W_win W_sub)
+        -- refactor
+        have mem_fst := W_sub (hg.has_pairing ⟨W, W_win⟩).mem_fst
+        rw [Finset.mem_filter] at mem_fst
+        have := Positional_Game_World.fst_colored_suffix H
+                  ((Positional_Game_World win_sets).hist_on_turn f_strat (Pairing_sStrat win_sets pairing) (n+1)).val
+                  Hsuf
+                  ((Positional_Game_World win_sets).hist_on_turn f_strat (Pairing_sStrat win_sets pairing) (n+1)).prop.1
+                  (pairing ⟨W, W_win⟩).1 (mem_fst.2)
+        dsimp [colored]
+        left
+        rw [this]
+        decide
+    )
+  simp_rw [Game_World_wDraw.hist_on_turn, Game_World.hist_on_turn_length] at this
+  exact this
+
+
+
+lemma there2 [Inhabited α] [DecidableEq α] [Fintype α] {win_sets : Finset (Finset α)} {pairing : win_sets → (α × α)}
+  (hg : Pairing_condition win_sets pairing) {n : Nat}
+  (f_strat : (Positional_Game_World win_sets).fStrategy)
+  (Neu : ∀ k ≤ n, Game_World_wDraw.state_on_turn_neutral (Positional_Game_World win_sets) f_strat (Pairing_sStrat win_sets pairing) k)
+  (H : List α) (Hsuf : H <:+ ((Positional_Game_World win_sets).hist_on_turn f_strat (Pairing_sStrat win_sets pairing) (n+1)).val )
+  (W : Finset α) (W_win : W ∈ win_sets) (W_sub : W ⊆ Finset.filter (fun x => State_from_history (fun _ => 0) (fun hist act => PosGame_trans (act :: hist)) (fun hist act => PosGame_trans (act :: hist)) H x = 1) Finset.univ)
+  {m : Nat} (mdef : WellFounded.min Nat.lt_wfRel.wf (colored pairing f_strat (pairing ⟨W, W_win⟩)) (colored_nonempty hg f_strat H Hsuf W W_win W_sub) = m+1)
+  : let M := WellFounded.min Nat.lt_wfRel.wf (colored pairing f_strat (pairing ⟨W, W_win⟩)) (colored_nonempty hg f_strat H Hsuf W W_win W_sub)
+  let Hi :=  (((Positional_Game_World win_sets).hist_on_turn f_strat (Pairing_sStrat win_sets pairing)))
+  (State_from_history (Positional_Game_World win_sets).toGame_World.init_game_state
+      (Positional_Game_World win_sets).toGame_World.fst_transition
+      (Positional_Game_World win_sets).toGame_World.snd_transition
+      (Hi M) (pairing ⟨W, W_win⟩).2 ≠ 0) →
+  Turn_fst M :=
+  by
+  intro M Hi S
+  dsimp [M]
+  rw [mdef]
+  have := Positional_Game_World.turn_fst_of_col_fst (Hi m).val (pairing ⟨W, W_win⟩).2
+    (by have := (Hi M).prop.1 ; rw [help_1_3_2 hg f_strat H Hsuf W W_win W_sub mdef S] at this ; exact this)
+    (almost2 hg f_strat H Hsuf W W_win W_sub mdef S)
+    (by rw [← Game_World_wDraw.state_on_turn_neutral_State_from_history_neutral]
+        apply Neu
+        rw [← Nat.succ_le_succ_iff, Nat.succ_eq_add_one, ← mdef]
+        apply  WellFounded.min_le Nat.lt_wfRel.wf _ (colored_nonempty hg f_strat H Hsuf W W_win W_sub)
+        -- refactor
+        have mem_fst := W_sub (hg.has_pairing ⟨W, W_win⟩).mem_fst
+        rw [Finset.mem_filter] at mem_fst
+        have := Positional_Game_World.fst_colored_suffix H
+                  ((Positional_Game_World win_sets).hist_on_turn f_strat (Pairing_sStrat win_sets pairing) (n+1)).val
+                  Hsuf
+                  ((Positional_Game_World win_sets).hist_on_turn f_strat (Pairing_sStrat win_sets pairing) (n+1)).prop.1
+                  (pairing ⟨W, W_win⟩).1 (mem_fst.2)
+        dsimp [colored]
+        left
+        rw [this]
+        decide
+    )
+  simp_rw [Game_World_wDraw.hist_on_turn, Game_World.hist_on_turn_length] at this
+  exact this
+
+
+lemma Hit_turn_is_neutral [Inhabited α] [DecidableEq α] [Fintype α] {win_sets : Finset (Finset α)} {pairing : win_sets → (α × α)}
+  (hg : Pairing_condition win_sets pairing) {n : Nat}
+  (f_strat : (Positional_Game_World win_sets).fStrategy)
+  (Neu : ∀ k ≤ n, Game_World_wDraw.state_on_turn_neutral (Positional_Game_World win_sets) f_strat (Pairing_sStrat win_sets pairing) k)
+  (H : List α) (Hsuf : H <:+ ((Positional_Game_World win_sets).hist_on_turn f_strat (Pairing_sStrat win_sets pairing) (n+1)).val )
+  (W : Finset α) (W_win : W ∈ win_sets) (W_sub : W ⊆ Finset.filter (fun x => State_from_history (fun _ => 0) (fun hist act => PosGame_trans (act :: hist)) (fun hist act => PosGame_trans (act :: hist)) H x = 1) Finset.univ)
+  : let M := WellFounded.min Nat.lt_wfRel.wf (colored pairing f_strat (pairing ⟨W, W_win⟩)) (colored_nonempty hg f_strat H Hsuf W W_win W_sub)
+  let Hi :=  (((Positional_Game_World win_sets).hist_on_turn f_strat (Pairing_sStrat win_sets pairing)))
+  State_from_history_neutral_wDraw (Positional_Game_World win_sets).toGame_World.init_game_state
+  (Positional_Game_World win_sets).toGame_World.fst_win_states
+  (Positional_Game_World win_sets).toGame_World.snd_win_states (Positional_Game_World win_sets).draw_states ↑(Hi M) :=
+  by
+  intro M Hi
+  have : M ≤ n+1 :=
+    by
+    apply  WellFounded.min_le Nat.lt_wfRel.wf _ (colored_nonempty hg f_strat H Hsuf W W_win W_sub)
+    -- refactor
+    have mem_fst := W_sub (hg.has_pairing ⟨W, W_win⟩).mem_fst
+    rw [Finset.mem_filter] at mem_fst
+    have := Positional_Game_World.fst_colored_suffix H
+              ((Positional_Game_World win_sets).hist_on_turn f_strat (Pairing_sStrat win_sets pairing) (n+1)).val
+              Hsuf
+              ((Positional_Game_World win_sets).hist_on_turn f_strat (Pairing_sStrat win_sets pairing) (n+1)).prop.1
+              (pairing ⟨W, W_win⟩).1 (mem_fst.2)
+    dsimp [colored]
+    left
+    rw [this]
+    decide
+  rw [le_iff_eq_or_lt] at this
+  cases' this with that that
+  · exfalso
+    have fst := W_sub (hg.has_pairing ⟨W,W_win⟩).mem_fst
+    have snd := W_sub (hg.has_pairing ⟨W,W_win⟩).mem_snd
+    rw [Finset.mem_filter] at fst snd
+    have but := second_uncolored hg f_strat H Hsuf W W_win W_sub
+      (by intro con
+          have one := Positional_Game_World.fst_colored_suffix _ _ Hsuf (Hi (n+1)).prop.1 (pairing ⟨W, W_win⟩).1 fst.2
+          rw [← that] at one
+          rw [one] at con
+          contradiction
+       )
+    have two := Positional_Game_World.fst_colored_suffix _ _ Hsuf (Hi (n+1)).prop.1 (pairing ⟨W, W_win⟩).2 snd.2
+    rw [← that] at two
+    rw [two] at but
+    contradiction
+  · rw [Nat.lt_succ] at that
+    rw [← Game_World_wDraw.state_on_turn_neutral_State_from_history_neutral]
+    apply Neu
+    exact that
+
+
+
+lemma Pairing_StratCore_colors_reacts_fst_consequemce [Inhabited α] [DecidableEq α] [Fintype α] {win_sets : Finset (Finset α)} {pairing : win_sets → (α × α)}
+  (hg : Pairing_condition win_sets pairing) {n : Nat}
+  (f_strat : (Positional_Game_World win_sets).fStrategy)
+  (Neu : ∀ k ≤ n, Game_World_wDraw.state_on_turn_neutral (Positional_Game_World win_sets) f_strat (Pairing_sStrat win_sets pairing) k)
+  (H : List α) (Hsuf : H <:+ ((Positional_Game_World win_sets).hist_on_turn f_strat (Pairing_sStrat win_sets pairing) (n+1)).val )
+  (W : Finset α) (W_win : W ∈ win_sets) (W_sub : W ⊆ Finset.filter (fun x => State_from_history (fun _ => 0) (fun hist act => PosGame_trans (act :: hist)) (fun hist act => PosGame_trans (act :: hist)) H x = 1) Finset.univ)
+  {m : Nat} (mdef : WellFounded.min Nat.lt_wfRel.wf (colored pairing f_strat (pairing ⟨W, W_win⟩)) (colored_nonempty hg f_strat H Hsuf W W_win W_sub) = m+1)
+  : let M := WellFounded.min Nat.lt_wfRel.wf (colored pairing f_strat (pairing ⟨W, W_win⟩)) (colored_nonempty hg f_strat H Hsuf W W_win W_sub)
+  let Hi :=  (((Positional_Game_World win_sets).hist_on_turn f_strat (Pairing_sStrat win_sets pairing)))
+  (State_from_history (Positional_Game_World win_sets).toGame_World.init_game_state
+      (Positional_Game_World win_sets).toGame_World.fst_transition
+      (Positional_Game_World win_sets).toGame_World.snd_transition
+      (Hi M) (pairing ⟨W, W_win⟩).1 ≠ 0) →
+  (State_from_history (Positional_Game_World win_sets).toGame_World.init_game_state
+      (Positional_Game_World win_sets).toGame_World.fst_transition
+      (Positional_Game_World win_sets).toGame_World.snd_transition
+      (Hi (M+1)) (pairing ⟨W, W_win⟩).2 = 2) :=
+  by
+  intro M Hi S
+  have T := there hg f_strat Neu H Hsuf W W_win W_sub mdef S
+  dsimp [M]
+  simp_rw [Turn_fst_not_step M] at T
+  rw [Game_World_wDraw.hist_on_turn, Game_World.hist_on_turn, dif_neg T]
+  dsimp
+  have RW := Pairing_StratCore_reacts_fst hg f_strat H Hsuf W W_win W_sub
+        (there hg f_strat Neu H Hsuf W W_win W_sub mdef S) S
+  dsimp [Pairing_sStrat]
+  dsimp [Game_World_wDraw.hist_on_turn] at RW
+  rw [RW]
+  apply Positional_Game_World.col_snd_of_turn_snd (Hi M).val (pairing ⟨W, W_win⟩).2
+    (by have := (Hi (M+1)).prop.1
+        simp_rw [Game_World_wDraw.hist_on_turn, Game_World.hist_on_turn, dif_neg T] at this
+        dsimp [Pairing_sStrat] at this
+        simp_rw [RW] at this
+        exact this
+    )
+    (by simp_rw [Game_World_wDraw.hist_on_turn, Game_World.hist_on_turn_length] ; apply T )
+    (by apply Hit_turn_is_neutral hg f_strat Neu H Hsuf W W_win W_sub
+    )
+
+
+
+lemma Pairing_StratCore_colors_reacts_snd_consequemce [Inhabited α] [DecidableEq α] [Fintype α] {win_sets : Finset (Finset α)} {pairing : win_sets → (α × α)}
+  (hg : Pairing_condition win_sets pairing) {n : Nat}
+  (f_strat : (Positional_Game_World win_sets).fStrategy)
+  (Neu : ∀ k ≤ n, Game_World_wDraw.state_on_turn_neutral (Positional_Game_World win_sets) f_strat (Pairing_sStrat win_sets pairing) k)
+  (H : List α) (Hsuf : H <:+ ((Positional_Game_World win_sets).hist_on_turn f_strat (Pairing_sStrat win_sets pairing) (n+1)).val )
+  (W : Finset α) (W_win : W ∈ win_sets) (W_sub : W ⊆ Finset.filter (fun x => State_from_history (fun _ => 0) (fun hist act => PosGame_trans (act :: hist)) (fun hist act => PosGame_trans (act :: hist)) H x = 1) Finset.univ)
+  {m : Nat} (mdef : WellFounded.min Nat.lt_wfRel.wf (colored pairing f_strat (pairing ⟨W, W_win⟩)) (colored_nonempty hg f_strat H Hsuf W W_win W_sub) = m+1)
+  : let M := WellFounded.min Nat.lt_wfRel.wf (colored pairing f_strat (pairing ⟨W, W_win⟩)) (colored_nonempty hg f_strat H Hsuf W W_win W_sub)
+  let Hi :=  (((Positional_Game_World win_sets).hist_on_turn f_strat (Pairing_sStrat win_sets pairing)))
+  (State_from_history (Positional_Game_World win_sets).toGame_World.init_game_state
+      (Positional_Game_World win_sets).toGame_World.fst_transition
+      (Positional_Game_World win_sets).toGame_World.snd_transition
+      (Hi M) (pairing ⟨W, W_win⟩).2 ≠ 0) →
+  (State_from_history (Positional_Game_World win_sets).toGame_World.init_game_state
+      (Positional_Game_World win_sets).toGame_World.fst_transition
+      (Positional_Game_World win_sets).toGame_World.snd_transition
+      (Hi (M+1)) (pairing ⟨W, W_win⟩).1 = 2) :=
+  by
+  intro M Hi S
+  have T := there2 hg f_strat Neu H Hsuf W W_win W_sub mdef S
+  dsimp [M]
+  simp_rw [Turn_fst_not_step M] at T
+  rw [Game_World_wDraw.hist_on_turn, Game_World.hist_on_turn, dif_neg T]
+  dsimp
+  have RW := Pairing_StratCore_reacts_snd hg f_strat H Hsuf W W_win W_sub
+        (there2 hg f_strat Neu H Hsuf W W_win W_sub mdef S) S
+  dsimp [Pairing_sStrat]
+  dsimp [Game_World_wDraw.hist_on_turn] at RW
+  rw [RW]
+  apply Positional_Game_World.col_snd_of_turn_snd (Hi M).val (pairing ⟨W, W_win⟩).1
+    (by have := (Hi (M+1)).prop.1
+        simp_rw [Game_World_wDraw.hist_on_turn, Game_World.hist_on_turn, dif_neg T] at this
+        dsimp [Pairing_sStrat] at this
+        simp_rw [RW] at this
+        exact this
+    )
+    (by simp_rw [Game_World_wDraw.hist_on_turn, Game_World.hist_on_turn_length] ; apply T )
+    (by apply Hit_turn_is_neutral hg f_strat Neu H Hsuf W W_win W_sub
+    )
+
+
+
+lemma Pairing_Strategy_Main_1 [Inhabited α] [DecidableEq α] [Fintype α] {win_sets : Finset (Finset α)} {pairing : win_sets → (α × α)}
+  (hg : Pairing_condition win_sets pairing) {n : Nat}
+  (f_strat : (Positional_Game_World win_sets).fStrategy)
+  (Neu : ∀ k ≤ n, Game_World_wDraw.state_on_turn_neutral (Positional_Game_World win_sets) f_strat (Pairing_sStrat win_sets pairing) k)
+  (H : List α) (Hsuf : H <:+ ((Positional_Game_World win_sets).hist_on_turn f_strat (Pairing_sStrat win_sets pairing) (n+1)).val )
+  (W : Finset α) (W_win : W ∈ win_sets) (W_sub : W ⊆ Finset.filter (fun x => State_from_history (fun _ => 0) (fun hist act => PosGame_trans (act :: hist)) (fun hist act => PosGame_trans (act :: hist)) H x = 1) Finset.univ)
+  {m : Nat} (mdef : WellFounded.min Nat.lt_wfRel.wf (colored pairing f_strat (pairing ⟨W, W_win⟩)) (colored_nonempty hg f_strat H Hsuf W W_win W_sub) = m+1)
+  : let M := WellFounded.min Nat.lt_wfRel.wf (colored pairing f_strat (pairing ⟨W, W_win⟩)) (colored_nonempty hg f_strat H Hsuf W W_win W_sub)
+  let Hi :=  (((Positional_Game_World win_sets).hist_on_turn f_strat (Pairing_sStrat win_sets pairing)))
+  (State_from_history (Positional_Game_World win_sets).toGame_World.init_game_state
+      (Positional_Game_World win_sets).toGame_World.fst_transition
+      (Positional_Game_World win_sets).toGame_World.snd_transition
+      (Hi M) (pairing ⟨W, W_win⟩).1 ≠ 0) →
+  False :=
+  by
+  intro M Hi S
+  by_cases Q : (n+1) ≤ M+1
+  · have su := List.IsSuffix.trans Hsuf (Game_World.hist_on_turn_suffix _ _ _ _ _ Q)
+    replace su := Positional_Game_World.fst_colored_suffix _ _ su (Hi (M+1)).prop.1 (pairing ⟨W, W_win⟩).2
+      (by have := W_sub (hg.has_pairing ⟨W,W_win⟩).mem_snd ; rw [Finset.mem_filter] at this ; exact this.2)
+    have fixHist := Pairing_StratCore_colors_reacts_fst_consequemce hg f_strat Neu H Hsuf W W_win W_sub mdef S
+    dsimp [Game_World_wDraw.hist_on_turn] at fixHist
+    rw [fixHist] at su
+    contradiction
+  · have su := (Game_World.hist_on_turn_suffix (Positional_Game_World win_sets).toGame_World f_strat (Pairing_sStrat win_sets pairing) _ _ (le_of_lt (not_le.mp Q)))
+    have one := Positional_Game_World.fst_colored_suffix _ _ Hsuf (Hi (n+1)).prop.1 (pairing ⟨W, W_win⟩).2
+      (by have := W_sub (hg.has_pairing ⟨W,W_win⟩).mem_snd ; rw [Finset.mem_filter] at this ; exact this.2)
+    have two := Positional_Game_World.snd_colored_suffix _ _ su (Hi (n+1)).prop.1 (pairing ⟨W, W_win⟩).2
+      (by apply Pairing_StratCore_colors_reacts_fst_consequemce hg f_strat Neu H Hsuf W W_win W_sub mdef S)
+    dsimp [Game_World_wDraw.hist_on_turn] at one
+    rw [one] at two
+    contradiction
+
+
+
+
+
+lemma Pairing_Strategy_Main_2 [Inhabited α] [DecidableEq α] [Fintype α] {win_sets : Finset (Finset α)} {pairing : win_sets → (α × α)}
+  (hg : Pairing_condition win_sets pairing) {n : Nat}
+  (f_strat : (Positional_Game_World win_sets).fStrategy)
+  (Neu : ∀ k ≤ n, Game_World_wDraw.state_on_turn_neutral (Positional_Game_World win_sets) f_strat (Pairing_sStrat win_sets pairing) k)
+  (H : List α) (Hsuf : H <:+ ((Positional_Game_World win_sets).hist_on_turn f_strat (Pairing_sStrat win_sets pairing) (n+1)).val )
+  (W : Finset α) (W_win : W ∈ win_sets) (W_sub : W ⊆ Finset.filter (fun x => State_from_history (fun _ => 0) (fun hist act => PosGame_trans (act :: hist)) (fun hist act => PosGame_trans (act :: hist)) H x = 1) Finset.univ)
+  {m : Nat} (mdef : WellFounded.min Nat.lt_wfRel.wf (colored pairing f_strat (pairing ⟨W, W_win⟩)) (colored_nonempty hg f_strat H Hsuf W W_win W_sub) = m+1)
+  : let M := WellFounded.min Nat.lt_wfRel.wf (colored pairing f_strat (pairing ⟨W, W_win⟩)) (colored_nonempty hg f_strat H Hsuf W W_win W_sub)
+  let Hi :=  (((Positional_Game_World win_sets).hist_on_turn f_strat (Pairing_sStrat win_sets pairing)))
+  (State_from_history (Positional_Game_World win_sets).toGame_World.init_game_state
+      (Positional_Game_World win_sets).toGame_World.fst_transition
+      (Positional_Game_World win_sets).toGame_World.snd_transition
+      (Hi M) (pairing ⟨W, W_win⟩).2 ≠ 0) →
+  False :=
+  by
+  intro M Hi S
+  by_cases Q : (n+1) ≤ M+1
+  · have su := List.IsSuffix.trans Hsuf (Game_World.hist_on_turn_suffix _ _ _ _ _ Q)
+    replace su := Positional_Game_World.fst_colored_suffix _ _ su (Hi (M+1)).prop.1 (pairing ⟨W, W_win⟩).1
+      (by have := W_sub (hg.has_pairing ⟨W,W_win⟩).mem_fst ; rw [Finset.mem_filter] at this ; exact this.2)
+    have fixHist := Pairing_StratCore_colors_reacts_snd_consequemce hg f_strat Neu H Hsuf W W_win W_sub mdef S
+    dsimp [Game_World_wDraw.hist_on_turn] at fixHist
+    rw [fixHist] at su
+    contradiction
+  · have su := (Game_World.hist_on_turn_suffix (Positional_Game_World win_sets).toGame_World f_strat (Pairing_sStrat win_sets pairing) _ _ (le_of_lt (not_le.mp Q)))
+    have one := Positional_Game_World.fst_colored_suffix _ _ Hsuf (Hi (n+1)).prop.1 (pairing ⟨W, W_win⟩).1
+      (by have := W_sub (hg.has_pairing ⟨W,W_win⟩).mem_fst ; rw [Finset.mem_filter] at this ; exact this.2)
+    have two := Positional_Game_World.snd_colored_suffix _ _ su (Hi (n+1)).prop.1 (pairing ⟨W, W_win⟩).1
+      (by apply Pairing_StratCore_colors_reacts_snd_consequemce hg f_strat Neu H Hsuf W W_win W_sub mdef S)
+    dsimp [Game_World_wDraw.hist_on_turn] at one
+    rw [one] at two
+    contradiction
+
+
+
+theorem Pairing_Strategy_Main [Inhabited α] [DecidableEq α] [Fintype α] {win_sets : Finset (Finset α)} {pairing : win_sets → (α × α)}
+  (hg : Pairing_condition win_sets pairing) {n : Nat}
+  (f_strat : (Positional_Game_World win_sets).fStrategy)
+  (Neu : ∀ k ≤ n, Game_World_wDraw.state_on_turn_neutral (Positional_Game_World win_sets) f_strat (Pairing_sStrat win_sets pairing) k)
+  (H : List α) (Hsuf : H <:+ ((Positional_Game_World win_sets).hist_on_turn f_strat (Pairing_sStrat win_sets pairing) (n+1)).val )
+  (W : Finset α) (W_win : W ∈ win_sets) (W_sub : W ⊆ Finset.filter (fun x => State_from_history (fun _ => 0) (fun hist act => PosGame_trans (act :: hist)) (fun hist act => PosGame_trans (act :: hist)) H x = 1) Finset.univ) :
+  False :=
+  by
+  let M := WellFounded.min Nat.lt_wfRel.wf (colored pairing f_strat (pairing ⟨W, W_win⟩)) (colored_nonempty hg f_strat H Hsuf W W_win W_sub)
+  by_cases Q : M = 0
+  · exfalso
+    exact (first_colored_turn_neq_zero hg f_strat H Hsuf W W_win W_sub) Q
+  · obtain ⟨m,mdef⟩ := Nat.succ_of_ne_zero Q
+    have M_mem := WellFounded.min_mem Nat.lt_wfRel.wf (colored pairing f_strat (pairing ⟨W, W_win⟩)) (colored_nonempty hg f_strat H Hsuf W W_win W_sub)
+    dsimp [colored] at M_mem
+    cases' M_mem with M_mem M_mem
+    · apply Pairing_Strategy_Main_1 hg f_strat Neu H Hsuf W W_win W_sub mdef M_mem
+    · apply Pairing_Strategy_Main_2 hg f_strat Neu H Hsuf W W_win W_sub mdef M_mem
+
+
+
+
+
+theorem Pairing_Strategy [Inhabited α] [DecidableEq α] [Fintype α] {win_sets : Finset (Finset α)} {pairing : win_sets → (α × α)}
+  (win_sets_nontrivial : ∅ ∉ win_sets) (hg : Pairing_condition win_sets pairing) :
+  (Positional_Game_World win_sets).is_draw_at_worst_snd :=
+  by
+  use Pairing_sStrat win_sets pairing
+  intro f_strat
+  obtain ⟨T,Tend,Tpre⟩ := Positional_Game_World.terminates win_sets win_sets_nontrivial f_strat (Pairing_sStrat win_sets pairing)
+  rw [Game_World_wDraw.state_on_turn_neutral, not_not] at Tend
+  cases' Tend with F S D
+  · exfalso
+    dsimp [Positional_Game_World] at F
+    obtain ⟨H, Hsuf, Hwin⟩ := F
+    obtain ⟨W,W_win, W_sub⟩ := Hwin
+    apply Pairing_Strategy_Main hg  f_strat Tpre H Hsuf W W_win W_sub
+  · left
+    use (T+1)
+    constructor
+    · apply S
+    · intro t tlT
+      rw [Nat.lt_succ] at tlT
+      exact Tpre t tlT
+  · right
+    use (T+1)
+    constructor
+    · apply D
+    · intro t tlT
+      rw [Nat.lt_succ] at tlT
+      exact Tpre t tlT
