Games/gameLib/Positional.lean
@@ -1,0 +1,481 @@
+/-
+Copyright (c) 2024 Yves Jäckle. All rights reserved.
+Released under Apache 2.0 license as described in the file LICENSE.
+Author: Yves Jäckle.
+-/
+
+import Games.gameLib.Termination
+import Games.gameLib.StateAPI
+import Games.gameLib.Playability
+
+
+/-
+This file describes a class of games know as positional games.
+Positional games are played on a finite set of elements, where each element
+may be claimed (or "colored") by either player. There is a set of subsets
+that are considered "winning sets". The first player to claim all all elements
+of a winning set (≈ monochromatic winning set) wins the game.
+An example of such a gam is Tic-tac-toe.
+
+The main concepts of this file are:
+- `Positional_Game_World` describes a `Game_World_wDraw` representing a positional game.
+- `Positional_Game_World.terminates` shows that positional games always terminate.
+-/
+
+
+/-- The color of the tile corresponds to the turn it was selcted on-/
+def PosGame_trans [DecidableEq α] (hist : List α) : α → Fin 3 :=
+  fun p => if  p ∈ hist
+           then if Turn_fst ((hist.reverse.indexOf p) + 1)
+                then 1
+                else 2
+           else 0
+
+
+
+/-- The first player wins if there is a winiing set colored entirely in `1`-/
+def PosGame_win_fst [DecidableEq α] [Fintype α] (win_sets : Finset (Finset α)) (ini : α → Fin 3) (hist : List α) : Prop :=
+  ∃ w ∈ win_sets, w ⊆ Finset.filter (fun x => (State_from_history ini (fun hist act => PosGame_trans (act :: hist)) (fun hist act => PosGame_trans (act :: hist)) hist) x = 1) Finset.univ
+
+/-- The second player wins if there is a winiing set colored entirely in `2`-/
+def PosGame_win_snd [DecidableEq α] [Fintype α] (win_sets : Finset (Finset α)) (ini : α → Fin 3) (hist : List α) : Prop :=
+  ∃ w ∈ win_sets, w ⊆ Finset.filter (fun x => (State_from_history ini (fun hist act => PosGame_trans (act :: hist)) (fun hist act => PosGame_trans (act :: hist)) hist) x = 2) Finset.univ
+
+
+
+
+open Classical
+
+
+/--
+A positional game is played o a board represented by a finite type α.
+We represent the players claiming tiles as follows: the state is `(s : α → Fin 3)`
+where tile `t` is claimed by the frist player if `s t = 1`, by the second player if
+`s t = 2`, and is unclaimed if `s t = 0`.
+
+Winning states corresond to monochromatic winning sets.
+The game is a draw if all tiles are colored (yet not winnig set is monochromatic).
+At each turn, a move (a tile) is legal to play if it wasn't claimed (ie. isn't in the history),
+and if all tiles are claimed (and the game is a draw), all moves are considered legal.
+-/
+def Positional_Game_World [DecidableEq α] [Fintype α] (win_sets : Finset (Finset α)) : Game_World_wDraw (α → Fin 3) α where
+     init_game_state := fun _ => 0
+     fst_transition := fun hist act => PosGame_trans (act :: hist)
+     snd_transition := fun hist act => PosGame_trans (act :: hist)
+     fst_win_states := fun hist => ∃ H, H <:+ hist ∧ PosGame_win_fst win_sets (fun _ => 0) H
+     snd_win_states := fun hist => ∃ H, H <:+ hist ∧ PosGame_win_snd win_sets (fun _ => 0) H
+     draw_states := fun hist => ∀ p : α, (State_from_history (fun _ => 0) (fun hist act => PosGame_trans (act :: hist)) (fun hist act => PosGame_trans (act :: hist)) hist) p ≠ 0
+     fst_legal := fun hist act =>
+                    if State_from_history_neutral_wDraw (fun _  : α => (0 : Fin 3)) -- for ↓ don't know why field names not accepted ... might be fixed when updating
+                         (fun hist => ∃ H, H <:+ hist ∧ PosGame_win_fst win_sets (fun _ => 0) H)
+                         (fun hist => ∃ H, H <:+ hist ∧ PosGame_win_snd win_sets (fun _ => 0) H)
+                         (fun hist => ∀ p : α, (State_from_history (fun _ => 0) (fun hist act => PosGame_trans (act :: hist)) (fun hist act => PosGame_trans (act :: hist)) hist) p ≠ 0)
+                         hist
+                    then act ∉ hist
+                    else True
+     snd_legal := fun hist act =>
+                    if State_from_history_neutral_wDraw (fun _ : α => (0 : Fin 3))
+                         (fun hist => ∃ H, H <:+ hist ∧ PosGame_win_fst win_sets (fun _ => 0) H)
+                         (fun hist => ∃ H, H <:+ hist ∧ PosGame_win_snd win_sets (fun _ => 0) H)
+                         (fun hist => ∀ p : α, (State_from_history (fun _ => 0) (fun hist act => PosGame_trans (act :: hist)) (fun hist act => PosGame_trans (act :: hist)) hist) p ≠ 0)
+                         hist
+                    then act ∉ hist
+                    else True
+
+
+
+
+lemma Positional_Game_World_mem_state [DecidableEq α] [Fintype α] (win_sets : Finset (Finset α)) (p : α) (hist : List α) (h : p ∈ hist) :
+     (State_from_history (Positional_Game_World win_sets).init_game_state (Positional_Game_World win_sets).fst_transition (Positional_Game_World win_sets).snd_transition hist) p ≠ 0 :=
+     by
+     cases' hist with x _
+     · contradiction
+     · dsimp [State_from_history, Positional_Game_World]
+       rw [ite_self]
+       dsimp [PosGame_trans]
+       rw [if_pos h]
+       split_ifs
+       all_goals {decide}
+
+lemma Positional_Game_World_mem_state' [DecidableEq α] [Fintype α] (win_sets : Finset (Finset α)) (p : α) (hist : List α)
+  (h : (State_from_history (Positional_Game_World win_sets).init_game_state (Positional_Game_World win_sets).fst_transition (Positional_Game_World win_sets).snd_transition hist) p ≠ 0) :
+    p ∈ hist :=
+    by
+    cases' hist with x _
+    · contradiction
+    · dsimp [State_from_history, Positional_Game_World] at h
+      rw [ite_self] at h
+      dsimp [PosGame_trans] at h
+      split_ifs at h
+      · rename_i m _
+        exact m
+      · rename_i m _
+        exact m
+      · contradiction
+
+
+
+lemma Positional_Game_World_playable [Inhabited α] [DecidableEq α] [Fintype α] (win_sets : Finset (Finset α)) : (Positional_Game_World win_sets).playable :=
+     by
+     intro hist _
+     constructor
+     · intro _
+       by_cases N : State_from_history_neutral_wDraw (Positional_Game_World win_sets).init_game_state (Positional_Game_World win_sets).fst_win_states (Positional_Game_World win_sets).snd_win_states (Positional_Game_World win_sets).draw_states hist
+       · dsimp [Positional_Game_World]
+         dsimp [Positional_Game_World] at N
+         simp_rw [if_pos N]
+         dsimp [State_from_history_neutral_wDraw] at N
+         replace N := N.2.2
+         push_neg at N
+         obtain ⟨p,pp⟩ := N
+         use p
+         contrapose! pp
+         apply Positional_Game_World_mem_state win_sets p hist pp
+       · use default
+         dsimp [Positional_Game_World]
+         dsimp [Positional_Game_World] at N
+         rw [if_neg N]
+         apply True.intro
+     · intro _
+       by_cases N : State_from_history_neutral_wDraw (Positional_Game_World win_sets).init_game_state (Positional_Game_World win_sets).fst_win_states (Positional_Game_World win_sets).snd_win_states (Positional_Game_World win_sets).draw_states hist
+       · dsimp [Positional_Game_World]
+         dsimp [Positional_Game_World] at N
+         simp_rw [if_pos N]
+         dsimp [State_from_history_neutral_wDraw] at N
+         replace N := N.2.2
+         push_neg at N
+         obtain ⟨p,pp⟩ := N
+         use p
+         contrapose! pp
+         apply Positional_Game_World_mem_state win_sets p hist pp
+       · use default
+         dsimp [Positional_Game_World]
+         dsimp [Positional_Game_World] at N
+         rw [if_neg N]
+         apply True.intro
+
+
+
+
+
+lemma Positional_Game_World.decreasing_neutral [DecidableEq α] [Fintype α] (win_sets : Finset (Finset α))
+  (hist Hist : List α)  (su : hist <:+ Hist) :
+  let g := Positional_Game_World win_sets
+  Finset.filter (fun x => (State_from_history g.init_game_state g.fst_transition g.snd_transition (Hist)) x = 0) Finset.univ
+  ⊆ Finset.filter (fun x => (State_from_history g.init_game_state g.fst_transition g.snd_transition (hist)) x = 0) Finset.univ :=
+  by
+  intro g
+  intro x
+  simp_rw [Finset.mem_filter]
+  rintro ⟨_,xdef⟩
+  refine' ⟨Finset.mem_univ _, _ ⟩
+  cases' Hist with y l
+  · rw [ List.suffix_nil] at su
+    rw [su]
+    exact xdef
+  · dsimp [State_from_history, Positional_Game_World] at xdef
+    rw [ite_self] at xdef
+    dsimp [PosGame_trans] at *
+    split_ifs at xdef
+    · contradiction
+    · contradiction
+    · rename_i main
+      cases' hist with z L
+      · dsimp [State_from_history, Positional_Game_World]
+      · dsimp [State_from_history, Positional_Game_World]
+        rw [ite_self]
+        unfold PosGame_trans
+        rw [if_neg (by contrapose! main ; exact List.mem_of_mem_suffix main su)]
+
+
+
+
+
+lemma Positional_Game_World.strict_decreasing_neutral [DecidableEq α] [Fintype α] (win_sets : Finset (Finset α))
+  (hist : List α) (act : α) :
+  let g := Positional_Game_World win_sets ;
+  g.hist_legal (act :: hist) →
+  State_from_history_neutral_wDraw g.init_game_state g.fst_win_states g.snd_win_states g.draw_states hist →
+  Finset.filter (fun x => (State_from_history g.init_game_state g.fst_transition g.snd_transition (act :: hist)) x = 0) Finset.univ
+  ⊂ Finset.filter (fun x => (State_from_history g.init_game_state g.fst_transition g.snd_transition (hist)) x = 0) Finset.univ :=
+  by
+  intro g leg N
+  rw [Finset.ssubset_iff_of_subset (Positional_Game_World.decreasing_neutral win_sets hist (act :: hist) (List.suffix_cons act hist))]
+  use act
+  simp_rw [Finset.mem_filter, Finset.mem_univ, true_and]
+  constructor
+  · cases' hist with x l
+    · dsimp [State_from_history, Positional_Game_World]
+    · dsimp [State_from_history, Positional_Game_World]
+      rw [ite_self]
+      dsimp [PosGame_trans]
+      cases' leg
+      rename_i now
+      split_ifs at now
+      · dsimp [g, Positional_Game_World] at now
+        rw [if_pos (by convert N)] at now
+        rw [if_neg now]
+      · dsimp [g, Positional_Game_World] at now
+        rw [if_pos (by convert N)] at now
+        rw [if_neg now]
+  · apply Positional_Game_World_mem_state
+    exact List.Mem.head hist
+
+
+
+
+lemma Positional_Game_World.draw_states_iff [DecidableEq α] [Fintype α] (win_sets : Finset (Finset α)) (hist : List α) :
+  let g := Positional_Game_World win_sets
+  (∀ p : α, (State_from_history g.init_game_state g.fst_transition g.snd_transition hist) p ≠ 0)
+  ↔  Finset.filter (fun x => (State_from_history g.init_game_state g.fst_transition g.snd_transition (hist)) x = 0) Finset.univ = ∅ :=
+  by
+  intro g
+  simp_rw [Finset.filter_eq_empty_iff, Finset.mem_univ, true_imp_iff]
+
+
+
+lemma Positional_Game_World.strict_decreasing_neutral_hists [DecidableEq α] [Fintype α] [Inhabited α] (win_sets : Finset (Finset α)) :
+  let g := Positional_Game_World win_sets ;
+  ∀ (f_strat : g.fStrategy), ∀ (s_strat : g.sStrategy),
+  ∀ n,
+  let H := (g.hist_on_turn f_strat s_strat)
+  State_from_history_neutral_wDraw g.init_game_state g.fst_win_states g.snd_win_states g.draw_states (H n) →
+  Finset.filter (fun x => (State_from_history g.init_game_state g.fst_transition g.snd_transition (H (n+1))) x = 0) Finset.univ
+  ⊂ Finset.filter (fun x => (State_from_history g.init_game_state g.fst_transition g.snd_transition (H n)) x = 0) Finset.univ :=
+  by
+  intro g f_strat s_strat n H N
+  have := (H (n+1)).prop.1
+  by_cases T : Turn_fst (n+1)
+  · dsimp [H, Game_World_wDraw.hist_on_turn, Game_World.hist_on_turn]
+    rw [dif_pos T]
+    dsimp [H, Game_World_wDraw.hist_on_turn, Game_World.hist_on_turn] at this
+    rw [dif_pos T] at this
+    apply Positional_Game_World.strict_decreasing_neutral win_sets _ _ this N
+  · dsimp [H, Game_World_wDraw.hist_on_turn, Game_World.hist_on_turn]
+    rw [dif_neg T]
+    dsimp [H, Game_World_wDraw.hist_on_turn, Game_World.hist_on_turn] at this
+    rw [dif_neg T] at this
+    apply Positional_Game_World.strict_decreasing_neutral win_sets _ _ this N
+
+
+
+lemma Positional_Game_World.fst_win_suffix [DecidableEq α] [Fintype α] [Inhabited α] (win_sets : Finset (Finset α))
+  (hist Hist : List α)  (su : hist <:+ Hist) :
+  let g := Positional_Game_World win_sets ;
+  g.fst_win_states hist → g.fst_win_states Hist :=
+  by
+  rintro g ⟨H,Hdef,X⟩
+  dsimp [g, Positional_Game_World] at *
+  use H
+  refine' ⟨List.IsSuffix.trans Hdef su,_⟩
+  exact X
+
+
+lemma Positional_Game_World.snd_win_suffix [DecidableEq α] [Fintype α] [Inhabited α] (win_sets : Finset (Finset α))
+  (hist Hist : List α)  (su : hist <:+ Hist) :
+  let g := Positional_Game_World win_sets ;
+  g.snd_win_states hist → g.snd_win_states Hist :=
+  by
+  rintro g ⟨H,Hdef,X⟩
+  dsimp [g, Positional_Game_World] at *
+  use H
+  refine' ⟨List.IsSuffix.trans Hdef su,_⟩
+  exact X
+
+lemma List.not_suffix_cons_nil {a : α} {l : List α} : ¬ (a :: l <:+ []) := by
+  simp_all only [suffix_nil, not_false_eq_true]
+
+lemma Positional_Game_World.draw_win_suffix [DecidableEq α] [Fintype α] [Inhabited α] (win_sets : Finset (Finset α))
+  (hist Hist : List α)  (su : hist <:+ Hist) :
+  let g := Positional_Game_World win_sets ;
+  g.draw_states hist → g.draw_states Hist :=
+  by
+  rintro g D
+  dsimp [g, Positional_Game_World] at *
+  intro p
+  specialize D p
+  contrapose! D
+  cases' hist with ah h
+  · dsimp [State_from_history]
+  · cases' Hist with aH H
+    · exfalso
+      exact List.not_suffix_cons_nil su
+    · dsimp [State_from_history] at *
+      rw [ite_self, PosGame_trans] at *
+      split_ifs at D
+      · contradiction
+      · contradiction
+      · rename_i main
+        rw [if_neg (by contrapose! main ; apply List.mem_of_mem_suffix main su )]
+
+
+
+
+lemma Positional_Game_World.neutral_of_suffix [DecidableEq α] [Fintype α] [Inhabited α] (win_sets : Finset (Finset α))
+  (hist Hist : List α)  (su : hist <:+ Hist) :
+  let g := Positional_Game_World win_sets ;
+  State_from_history_neutral_wDraw g.init_game_state g.fst_win_states g.snd_win_states g.draw_states Hist
+  → State_from_history_neutral_wDraw g.init_game_state g.fst_win_states g.snd_win_states g.draw_states hist :=
+  by
+  rintro g ⟨Nf, Ns,Nd⟩
+  constructor
+  · contrapose! Nf
+    apply Positional_Game_World.fst_win_suffix _ _ _ su Nf
+  · constructor
+    · contrapose! Ns
+      apply Positional_Game_World.snd_win_suffix _ _ _ su Ns
+    · contrapose! Nd
+      apply Positional_Game_World.draw_win_suffix _ _ _ su Nd
+
+
+
+
+lemma Positional_Game_World.terminates [DecidableEq α] [Fintype α] [Inhabited α] (win_sets : Finset (Finset α))
+  (win_sets_nontrivial : ∅ ∉ win_sets) :
+  let g := Positional_Game_World win_sets ;
+  ∀ (f_strat : g.fStrategy), ∀ (s_strat : g.sStrategy),
+  ∃ n, ¬ Game_World_wDraw.state_on_turn_neutral g f_strat s_strat (n+1) ∧
+    ∀ m ≤ n, Game_World_wDraw.state_on_turn_neutral g f_strat s_strat m :=
+  by
+  intro g f_strat s_strat
+  let N := {s | ∃ n,
+      let H := (g.hist_on_turn f_strat s_strat n)
+      s = Finset.filter (fun x => (State_from_history g.init_game_state g.fst_transition g.snd_transition H) x = 0) Finset.univ
+      ∧ State_from_history_neutral_wDraw g.init_game_state g.fst_win_states g.snd_win_states g.draw_states H}
+  have N_nonempty : Set.Nonempty N := by
+    use Finset.filter (fun x => (State_from_history g.init_game_state g.fst_transition g.snd_transition (g.hist_on_turn f_strat s_strat 0)) x = 0) Finset.univ
+    use 0
+    intro H
+    constructor
+    · rfl
+    · dsimp [H, Game_World_wDraw.hist_on_turn, Game_World.hist_on_turn, State_from_history_neutral_wDraw, Positional_Game_World]
+      constructor
+      · intro con
+        obtain ⟨H,Hdef,X⟩ := con
+        rw [List.suffix_nil] at Hdef
+        rw [Hdef] at X
+        obtain ⟨oh,no,pe⟩ := X
+        dsimp [State_from_history] at pe
+        rw [Finset.filter_false_of_mem (fun _ _ => by decide), Finset.subset_empty] at pe
+        rw [pe] at no
+        exact win_sets_nontrivial no
+      · constructor
+        · intro con
+          obtain ⟨H,Hdef,X⟩ := con
+          rw [List.suffix_nil] at Hdef
+          rw [Hdef] at X
+          obtain ⟨oh,no,pe⟩ := X
+          dsimp [State_from_history] at pe
+          rw [Finset.filter_false_of_mem (fun _ _ => by decide), Finset.subset_empty] at pe
+          rw [pe] at no
+          exact win_sets_nontrivial no
+        · intro con
+          apply con Inhabited.default
+          dsimp [State_from_history]
+  obtain ⟨n,ndef,ne⟩ := WellFounded.min_mem Finset.isWellFounded_ssubset.wf N N_nonempty
+  use n
+  constructor
+  · intro con
+    rw [Game_World_wDraw.state_on_turn_neutral_State_from_history_neutral] at con
+    apply @WellFounded.not_lt_min _ _ Finset.isWellFounded_ssubset.wf N N_nonempty
+        (Finset.filter (fun x => (State_from_history g.init_game_state g.fst_transition g.snd_transition (g.hist_on_turn f_strat s_strat (n+1))) x = 0) Finset.univ)
+        (by use n+1 )
+    rw [ndef]
+    apply Positional_Game_World.strict_decreasing_neutral_hists
+    apply ne
+  · intro m mln
+    rw [Game_World_wDraw.state_on_turn_neutral_State_from_history_neutral]
+    apply Positional_Game_World.neutral_of_suffix _ _ (g.hist_on_turn f_strat s_strat n).val
+    · dsimp [Game_World_wDraw.hist_on_turn]
+      apply Game_World.hist_on_turn_suffix
+      exact mln
+    · exact ne
+
+
+
+lemma Positional_Game_World.col_fst_of_turn_fst [DecidableEq α] [Fintype α] [Inhabited α] {win_sets : Finset (Finset α)}
+  (hist : List α) (act : α) (leg : (Positional_Game_World win_sets).hist_legal (act :: hist))
+  (ts : Turn_fst (hist.length + 1)) :
+  let g := (Positional_Game_World win_sets) ;
+  State_from_history_neutral_wDraw g.init_game_state g.fst_win_states g.snd_win_states g.draw_states (hist) →
+  (State_from_history g.init_game_state g.fst_transition  g.snd_transition (act :: hist)) act = 1 :=
+  by
+  intro g N
+  dsimp [State_from_history]
+  rw [if_pos ts]
+  dsimp [Positional_Game_World, PosGame_trans]
+  rw [if_pos (by apply List.mem_cons_self)]
+  cases' leg
+  rename_i _ now
+  rw [if_pos ts] at now
+  dsimp [Positional_Game_World] at now
+  rw [if_pos (by  convert N), ← List.mem_reverse] at now
+  rw [if_pos (by rw [List.reverse_cons, List.indexOf_append_of_not_mem now, List.length_reverse, List.indexOf_cons_eq _ rfl] ; exact ts)]
+
+
+
+
+
+
+lemma Positional_Game_World.col_snd_of_turn_snd [DecidableEq α] [Fintype α] [Inhabited α] {win_sets : Finset (Finset α)}
+  (hist : List α) (act : α) (leg : (Positional_Game_World win_sets).hist_legal (act :: hist))
+  (ts : ¬ Turn_fst (hist.length + 1)) :
+  let g := (Positional_Game_World win_sets) ;
+  State_from_history_neutral_wDraw g.init_game_state g.fst_win_states g.snd_win_states g.draw_states (hist) →
+  (State_from_history g.init_game_state g.fst_transition  g.snd_transition (act :: hist)) act = 2 :=
+  by
+  intro g N
+  dsimp [State_from_history]
+  rw [if_neg ts]
+  dsimp [Positional_Game_World, PosGame_trans]
+  rw [if_pos (by apply List.mem_cons_self)]
+  cases' leg
+  rename_i _ now
+  rw [if_neg ts] at now
+  dsimp [Positional_Game_World] at now
+  rw [if_pos (by  convert N), ← List.mem_reverse] at now
+  rw [if_neg (by rw [List.reverse_cons, List.indexOf_append_of_not_mem now, List.length_reverse, List.indexOf_cons_eq _ rfl] ; exact ts)]
+
+
+lemma Positional_Game_World.turn_fst_of_col_fst [DecidableEq α] [Fintype α] [Inhabited α] {win_sets : Finset (Finset α)}
+  (hist : List α) (act : α) (leg : (Positional_Game_World win_sets).hist_legal (act :: hist)) :
+  let g := (Positional_Game_World win_sets) ;
+  (State_from_history g.init_game_state g.fst_transition  g.snd_transition (act :: hist)) act = 1 →
+  State_from_history_neutral_wDraw g.init_game_state g.fst_win_states g.snd_win_states g.draw_states (hist) →
+  Turn_fst (hist.length + 1) :=
+  by
+  intro g S N
+  by_contra con
+  dsimp [State_from_history] at S
+  rw [if_neg con] at S
+  dsimp [Positional_Game_World, PosGame_trans] at S
+  rw [if_pos (by apply List.mem_cons_self)] at S
+  cases' leg
+  rename_i _ now
+  rw [if_neg con] at now
+  dsimp [Positional_Game_World] at now
+  rw [if_pos (by  convert N), ← List.mem_reverse] at now
+  rw [if_neg (by rw [List.reverse_cons, List.indexOf_append_of_not_mem now, List.length_reverse, List.indexOf_cons_eq _ rfl] ; exact con)] at S
+  contradiction
+
+
+
+lemma Positional_Game_World.turn_snd_of_col_snd [DecidableEq α] [Fintype α] [Inhabited α] {win_sets : Finset (Finset α)}
+  (hist : List α) (act : α) (leg : (Positional_Game_World win_sets).hist_legal (act :: hist)) :
+  let g := (Positional_Game_World win_sets) ;
+  (State_from_history g.init_game_state g.fst_transition  g.snd_transition (act :: hist)) act = 2 →
+  State_from_history_neutral_wDraw g.init_game_state g.fst_win_states g.snd_win_states g.draw_states (hist) →
+  ¬ Turn_fst (hist.length + 1) :=
+  by
+  intro g S N con
+  dsimp [State_from_history] at S
+  rw [if_pos con] at S
+  dsimp [Positional_Game_World, PosGame_trans] at S
+  rw [if_pos (by apply List.mem_cons_self)] at S
+  cases' leg
+  rename_i _ now
+  rw [if_pos con] at now
+  dsimp [Positional_Game_World] at now
+  rw [if_pos (by  convert N), ← List.mem_reverse] at now
+  rw [if_pos (by rw [List.reverse_cons, List.indexOf_append_of_not_mem now, List.length_reverse, List.indexOf_cons_eq _ rfl] ; exact con)] at S
+  contradiction
