Games/games/TicTacToe.lean
@@ -1,0 +1,272 @@
+/-
+Copyright (c) 2024 Yves Jäckle. All rights reserved.
+Released under Apache 2.0 license as described in the file LICENSE.
+Author: Yves Jäckle.
+-/
+
+import Games.gameLib.Pairing
+import Games.games.TTT_CombinatorialLines
+
+
+
+/-
+This file desribes the game of Tic-tac-toe ... in high dimension !
+The games is played of the gridpoints of a D dimensional cube of length n.
+Players color gridpoints turn by turn. The first player to color an entire
+combinatorial line by their color wins the game. A combinatorial line is a
+set of gridpoints such that for each coordinate, the points form either
+an increasing (0,1,...,n-1), increasing (n-1,n-2,...,0), or constant
+sequence (and not all sequences are constant).
+
+Using Hall's theorem, we'll show that if `n ≥ 3^D - 1`, Tic-tac-toe allows for
+a paring strategy for the players, so that it ends in a draw in the worst case
+for either one.
+
+The main concepts of the file are:
+- `TTT_win_sets` descrbe the winnig sets of Tic-tac-toe, so that it may be described
+  as a positional game.
+- `Hall_condition` derives the condition to Hall's theorem from the bound `n ≥ 3^D - 1`
+- `TTT_Pairing_condition` shows that Tic-tac-toe satisfies the pairing conditions if `n ≥ 3^D - 1`
+- `TTT_is_draw_at_worst_snd` shows that Tic-tac-toe has a drawinf strategy for the second player.
+
+-/
+
+variable (D n : ℕ)
+
+variable (hn : 1 < n)
+
+open Classical
+
+noncomputable
+def TTT_win_sets : Finset (Finset (Fin D → Fin n)) := Finset.univ.filter (is_combi_line D n (strengthen n hn))
+
+noncomputable
+def TTT := Positional_Game_World (TTT_win_sets D n hn)
+
+#check incidence_ub
+
+#check  Finset.all_card_le_biUnion_card_iff_existsInjective'
+#check Fintype.all_card_le_rel_image_card_iff_exists_injective
+
+#check Finset.biUnion
+
+
+noncomputable
+instance : Finite ({c : Finset (Fin D → Fin n) // is_combi_line D n (strengthen n hn) c} × Bool) := by infer_instance
+
+noncomputable
+instance : Fintype ({c : Finset (Fin D → Fin n) // is_combi_line D n (strengthen n hn) c} × Bool) := by infer_instance
+
+
+def line_set_neighbours (l : {c : Finset (Fin D → Fin n) // is_combi_line D n (strengthen n hn) c} × Bool): Finset (Fin D → Fin n) :=
+  Finset.univ.filter (fun p => p ∈ l.1.val)
+
+noncomputable
+def point_neighbours (p : Fin D → Fin n): Finset ({c : Finset (Fin D → Fin n) // is_combi_line D n (strengthen n hn) c} × Bool) :=
+  Finset.univ.filter (fun l => p ∈ l.1.val)
+
+def line_point_rel (l : {c : Finset (Fin D → Fin n) // is_combi_line D n (strengthen n hn) c} × Bool) (p : Fin D → Fin n) : Prop  := p ∈ l.1.val
+
+#check Finset.sum_card_bipartiteAbove_eq_sum_card_bipartiteBelow
+
+lemma double_count_line_points (ls : Finset ({c : Finset (Fin D → Fin n) // is_combi_line D n (strengthen n hn) c} × Bool)) :
+  (Finset.sum ls (fun a => (Finset.bipartiteAbove (line_point_rel D n hn) (Finset.biUnion ls (line_set_neighbours D n hn)) a).card)) =
+  Finset.sum (Finset.biUnion ls (line_set_neighbours D n hn)) (fun b => (Finset.bipartiteBelow (line_point_rel D n hn) ls b).card) :=
+  @Finset.sum_card_bipartiteAbove_eq_sum_card_bipartiteBelow _ _  (line_point_rel D n hn) ls (Finset.biUnion ls (line_set_neighbours D n hn)) _
+
+
+lemma line_has_n_points (ls : Finset ({c : Finset (Fin D → Fin n) // is_combi_line D n (strengthen n hn) c} × Bool)) (a : {c : Finset (Fin D → Fin n) // is_combi_line D n (strengthen n hn) c} × Bool) (ha : a ∈ ls) :
+  (Finset.bipartiteAbove (line_point_rel D n hn) (Finset.biUnion ls (line_set_neighbours D n hn)) a).card = n :=
+  by
+  dsimp [Finset.bipartiteAbove]
+  have : Finset.filter (line_point_rel D n hn a) (Finset.biUnion ls (line_set_neighbours D n hn)) = Finset.univ.filter (fun p => p ∈ a.1.val) :=
+    by
+    ext x
+    simp_rw [Finset.mem_filter]
+    rw [Finset.mem_biUnion, line_point_rel]
+    constructor
+    · rintro ⟨_,m⟩
+      exact ⟨Finset.mem_univ _, m⟩
+    · rintro ⟨_,m⟩
+      constructor
+      · use a
+        rw [line_set_neighbours, Finset.mem_filter]
+        exact ⟨ha, Finset.mem_univ _, m⟩
+      · exact m
+  rw [this]
+  clear this
+  obtain ⟨s,sdef, sim⟩ := a.1.prop
+  rw [sim, Finset.filter_mem_image_eq_image _ _ _ (fun _ _ => Finset.mem_univ _)]
+  simp_rw [← Finset.card_fin n, Finset.card_image_iff]
+  apply seq_inj D n hn s sdef
+
+#check Finset.card_image_iff
+
+#check Finset.card_fin
+
+-- to mathlib ?
+lemma Finset.card_filter_le_card_filter_univ [Fintype α ]
+  {s : Finset α} {p : α → Prop} [DecidablePred p] : (s.filter p).card ≤ (Finset.univ.filter p).card :=
+  by
+  apply Finset.card_le_card
+  apply Finset.filter_subset_filter
+  exact subset_univ s
+
+lemma point_inicdence_ub (ls : Finset ({c : Finset (Fin D → Fin n) // is_combi_line D n (strengthen n hn) c} × Bool)) (p : Fin D → Fin n) :
+  (Finset.bipartiteBelow (line_point_rel D n hn) ls p).card ≤ (3^D - 1) :=
+  by
+  apply le_trans _ (Nat.mul_div_le _ 2)
+  have : (Finset.bipartiteBelow (line_point_rel D n hn) ls p).card ≤ ((Finset.univ : Finset Bool) ×ˢ (Finset.filter (fun c => is_combi_line D n (strengthen n hn) c ∧ p ∈ c) Finset.univ)).card :=
+    by
+    apply le_trans (Finset.card_filter_le_card_filter_univ)
+    apply Finset.card_le_card_of_inj_on (fun x : ({c : Finset (Fin D → Fin n) // is_combi_line D n (strengthen n hn) c} × Bool) => (x.2, x.1.val))
+    · simp_rw [Finset.mem_filter, Finset.mem_product,Finset.mem_filter]
+      rintro a ⟨ _, h ⟩
+      refine' ⟨Finset.mem_univ _, Finset.mem_univ _, _ ⟩
+      constructor
+      · exact a.1.prop
+      · apply h
+    · intro a _ b _ main
+      rw [Prod.eq_iff_fst_eq_snd_eq]
+      simp_rw [Prod.eq_iff_fst_eq_snd_eq] at main
+      exact ⟨Subtype.eq main.2, main.1⟩
+  apply le_trans this
+  rw [Finset.card_product, Finset.card_univ,  Fintype.card_bool]
+  apply Nat.mul_le_mul_left
+  apply incidence_ub D n hn
+
+
+
+lemma main_bound (ls : Finset ({c : Finset (Fin D → Fin n) // is_combi_line D n (strengthen n hn) c} × Bool)) :  ls.card * n ≤ (Finset.biUnion ls (line_set_neighbours D n hn)).card * (3^D - 1) :=
+  by
+  simp_rw [Finset.card_eq_sum_ones, Finset.sum_mul, one_mul]
+  have := double_count_line_points D n hn ls
+  have L : (Finset.sum ls fun a => (Finset.bipartiteAbove (line_point_rel D n hn) (Finset.biUnion ls (line_set_neighbours D n hn)) a).card) = (Finset.sum ls fun _ => n) :=
+    by
+    apply Finset.sum_congr rfl (fun x hx => line_has_n_points D n hn ls x hx)
+  have R : Finset.sum (Finset.biUnion ls (line_set_neighbours D n hn)) (fun b => (Finset.bipartiteBelow (line_point_rel D n hn) ls b).card) ≤ Finset.sum (Finset.biUnion ls (line_set_neighbours D n hn)) (fun x => 3 ^ D - 1) :=
+    by
+    apply Finset.sum_le_sum
+    intro a _
+    apply point_inicdence_ub
+  apply le_trans _ R
+  rw [← L]
+  apply le_of_eq
+  exact this
+
+
+
+lemma Hall_condition (ls : Finset ({c : Finset (Fin D → Fin n) // is_combi_line D n (strengthen n hn) c} × Bool))
+  (h : n ≥ 3^D - 1) :
+  ls.card ≤ (Finset.biUnion ls (line_set_neighbours D n hn)).card :=
+  by
+  have := main_bound D n hn ls
+  apply Nat.le_of_mul_le_mul_left _ (show 0 < n by apply lt_trans _ hn ; exact Nat.one_pos)
+  rw [mul_comm]
+  apply le_trans this
+  rw [mul_comm]
+  apply Nat.mul_le_mul_right
+  exact h
+
+
+
+variable (h : n ≥ 3^D - 1)
+
+noncomputable
+def pre_TTT_pairing  :=
+  Classical.choose ((Finset.all_card_le_biUnion_card_iff_existsInjective' (line_set_neighbours D n hn)).mp (fun ls => Hall_condition D n hn ls h))
+
+lemma pre_TTT_pairing_inj : Function.Injective (pre_TTT_pairing D n hn h) :=
+  (Classical.choose_spec ((Finset.all_card_le_biUnion_card_iff_existsInjective' (line_set_neighbours D n hn)).mp (fun ls => Hall_condition D n hn ls h))).1
+
+lemma pre_TTT_pairing_map (l : { c // is_combi_line D n (strengthen n hn) c } × Bool) :
+  (pre_TTT_pairing D n hn h) l ∈ (line_set_neighbours D n hn) l :=
+  (Classical.choose_spec ((Finset.all_card_le_biUnion_card_iff_existsInjective' (line_set_neighbours D n hn)).mp (fun ls => Hall_condition D n hn ls h))).2 l
+
+
+lemma line_set_neighbours_is_line (l : {c : Finset (Fin D → Fin n) // is_combi_line D n (strengthen n hn) c} × Bool) :
+  line_set_neighbours D n hn l = l.1.val :=
+  by
+  dsimp [line_set_neighbours]
+  rw [Finset.filter_univ_mem]
+
+
+noncomputable
+def TTT_pairing : (TTT_win_sets D n hn) → ((Fin D → Fin n) × (Fin D → Fin n)) :=
+  fun w =>
+    let w_dtt_pain := (⟨w.val, by have wp := w.prop ; simp_rw [TTT_win_sets, Finset.mem_filter, Finset.mem_univ, true_and] at wp ; exact wp ⟩ : {x // is_combi_line D n (strengthen n hn) x})
+    (pre_TTT_pairing D n hn h (w_dtt_pain, true), pre_TTT_pairing D n hn h (w_dtt_pain, false))
+
+
+lemma TTT_Pairing_condition : Pairing_condition (TTT_win_sets D n hn) (TTT_pairing D n hn h) where
+  has_pairing := by
+    intro w
+    let w_dtt_pain := (⟨w.val, by have wp := w.prop ; simp_rw [TTT_win_sets, Finset.mem_filter, Finset.mem_univ, true_and] at wp ; exact wp ⟩ : {x // is_combi_line D n (strengthen n hn) x})
+    rw [TTT_pairing]
+    constructor
+    · dsimp
+      intro con
+      have := pre_TTT_pairing_inj D n hn h con
+      simp_rw [Prod.eq_iff_fst_eq_snd_eq] at this
+      exact this.2
+    · dsimp
+      have := pre_TTT_pairing_map D n hn h (w_dtt_pain, true)
+      rw [line_set_neighbours_is_line] at this
+      apply this
+    · dsimp
+      have := pre_TTT_pairing_map D n hn h (w_dtt_pain, false)
+      rw [line_set_neighbours_is_line] at this
+      apply this
+  pairing_dif := by
+    intro w v wnv
+    dsimp [TTT_pairing]
+    constructor
+    · intro con
+      dsimp at con
+      replace con := pre_TTT_pairing_inj D n hn h con
+      rw [Prod.eq_iff_fst_eq_snd_eq] at con
+      apply wnv
+      apply Subtype.eq
+      dsimp at con
+      rw [← Subtype.val_inj] at con
+      apply con.1
+    · intro con
+      dsimp at con
+      replace con := pre_TTT_pairing_inj D n hn h con
+      rw [Prod.eq_iff_fst_eq_snd_eq] at con
+      apply wnv
+      apply Subtype.eq
+      dsimp at con
+      rw [← Subtype.val_inj] at con
+      apply con.1
+    · intro con
+      dsimp at con
+      replace con := pre_TTT_pairing_inj D n hn h con
+      rw [Prod.eq_iff_fst_eq_snd_eq] at con
+      dsimp at con
+      apply Bool.noConfusion con.2
+    · intro con
+      dsimp at con
+      replace con := pre_TTT_pairing_inj D n hn h con
+      rw [Prod.eq_iff_fst_eq_snd_eq] at con
+      dsimp at con
+      apply Bool.noConfusion con.2
+
+lemma TTT_win_sets_nontrivial : ∅ ∉ (TTT_win_sets D n hn) :=
+  by
+  intro con
+  rw [TTT_win_sets, Finset.mem_filter] at con
+  obtain ⟨seq,_,seqp⟩ := con.2
+  apply Finset.not_mem_empty (seq ⟨0,by rw [Nat.pos_iff_ne_zero] ; exact (strengthen n hn) ⟩)
+  rw [seqp]
+  rw [Finset.mem_image]
+  use ⟨0,by rw [Nat.pos_iff_ne_zero] ; exact (strengthen n hn) ⟩
+  exact ⟨Finset.mem_univ _ , rfl⟩
+
+
+
+instance speInst : Inhabited (Fin D → Fin n) where default := (fun _ => ⟨0, lt_trans zero_lt_one hn ⟩ )
+
+theorem TTT_is_draw_at_worst_snd : (TTT D n hn).is_draw_at_worst_snd :=
+  by
+  exact @Pairing_Strategy _ (speInst D n hn) _ _ _ _ (TTT_win_sets_nontrivial D n hn) (TTT_Pairing_condition D n hn h)
